Small sets library to express point free set reasoning for generators semantics.
Rewrote most of the proofs in GenLow.
Had to admit some in GenHigh and SemChecker, working on it.

The biggest change I made was that generators are now nat -> RandomSeed -> T
instead of RandomSeed -> nat -> T which makes it easier to use the monad
operators with explicit sizes. It may have broken other things though.

src/GenLow.v
@@ -1,34 +1,24 @@
-Require Import ZArith List ssreflect ssrbool ssrnat.
+Require Import ZArith List ssreflect ssrfun ssrbool ssrnat.
 Require Import Random RoseTrees.
-Require Import Ensembles.
+Require Import Sets.
 Require Import Numbers.BinNums.
 Require Import Classes.RelationClasses.
 
 Set Implicit Arguments.
+Unset Strict Implicit.
+Unset Printing Implicit Defensive.
 
 Import ListNotations.
 
 (* Low-level Generators *)
 
-(* There are similar definitions in the Ensembles library (Included
-   and Same_set); set_eq is not exactly the same as Same_set though
-   (only logically equivalent). *)
-Definition set_eq {A} (m1 m2 : Ensemble A) :=
-  forall (a : A), m1 a <-> m2 a.
+Open Scope fun_scope.
+Open Scope set_scope.
 
-Global Instance : forall A, Equivalence (@set_eq A).
+Lemma randomSplit_codom : codom randomSplit <--> setT.
 Proof.
-admit.
+by apply/subset_eqP; split=> // [[s1 s2]] _; apply: randomSplitAssumption.
 Qed.
-
-Infix "<-->" := set_eq (at level 70, no associativity) : sem_gen_scope.
-
-Definition set_incl {A} (m1 m2 : Ensemble A) :=
-  forall (a : A), m1 a -> m2 a.
-
-Infix "--->" := set_incl (at level 70, no associativity) : sem_gen_scope.
-
-Open Scope sem_gen_scope.
 
 (* We hide the implementation of generators behind this interface. The
    rest of the framework and user code are agnostic to the internal
@@ -36,413 +26,321 @@ Open Scope sem_gen_scope.
    tries to follow this code organization/abstraction. We need to
    expose quite a bit on the proof side for this to work though. *)
 Module Type GenLowInterface.
-   Parameter G : Type -> Type.
+Parameter G : Type -> Type.
 
-   (* Standard (primitive) generator interface *)
-   Parameter returnGen  : forall {A : Type}, A -> G A.
-   Parameter bindGen :  forall {A B : Type}, G A -> (A -> G B) -> G B.
-   Parameter run  : forall {A : Type}, G A -> RandomSeed -> nat -> A.
-   Parameter fmap : forall {A B : Type}, (A -> B) -> G A -> G B.
-   Parameter sized : forall {A: Type}, (nat -> G A) -> G A.
-   Parameter resize : forall {A: Type}, nat -> G A -> G A.
-   Parameter promote : forall {A : Type}, Rose (G A) -> G (Rose A).
-   Parameter suchThatMaybe : forall {A : Type}, G A -> (A -> bool) ->
-                                                G (option A).
-   Parameter choose : forall {A : Type} `{Random A}, (A * A) -> G A.
-   Parameter sample : forall {A : Type}, G A -> list A.
+(* Standard (primitive) generator interface *)
+Parameter returnGen  : forall {A : Type}, A -> G A.
+Parameter bindGen :  forall {A B : Type}, G A -> (A -> G B) -> G B.
+Parameter run  : forall {A : Type}, G A -> nat -> RandomSeed -> A.
+Parameter fmap : forall {A B : Type}, (A -> B) -> G A -> G B.
+Parameter sized : forall {A: Type}, (nat -> G A) -> G A.
+Parameter resize : forall {A: Type}, nat -> G A -> G A.
+Parameter promote : forall {A : Type}, Rose (G A) -> G (Rose A).
+Parameter suchThatMaybe : forall {A : Type}, G A -> (A -> bool) ->
+                                             G (option A).
+Parameter choose : forall {A : Type} `{Random A}, (A * A) -> G A.
+Parameter sample : forall {A : Type}, G A -> list A.
 
 (* LL: The abstraction barrier is annoying :D *)
-   Parameter variant : forall {A : Type}, SplitPath -> G A -> G A.
-   Parameter reallyUnsafePromote : forall {r A:Type}, (r -> G A) -> G (r -> A).
+Parameter variant : forall {A : Type}, SplitPath -> G A -> G A.
+Parameter reallyUnsafePromote : forall {r A:Type}, (r -> G A) -> G (r -> A).
 
-   (* Set of outcomes semantics definitions (repeated below) *)
-   Definition semGenSize {A : Type} (g : G A) (size : nat) : Ensemble A :=
-     fun a => exists seed, run g seed size = a.
-   Definition semGen {A : Type} (g : G A) : Ensemble A :=
-     fun a => exists size, semGenSize g size a.
+(* Set of outcomes semantics definitions (repeated below) *)
+Definition semGenSize {A : Type} (g : G A) (size : nat) : set A :=
+  codom (run g size).
+Definition semGen {A : Type} (g : G A) : set A :=
+  \bigcup_size semGenSize g size.
 
+Hypothesis semReturn :
+  forall A (x : A), semGen (returnGen x) <--> [set x].
+Hypothesis semReturnSize :
+  forall A size (x : A), semGenSize (returnGen x) size <--> [set x].
 
-   Hypothesis semReturn :
-     forall A (x : A), semGen (returnGen x) <--> eq x.
-   Hypothesis semReturnSize :
-     forall A (x : A) (size : nat), semGenSize (returnGen x) size <--> eq x.
+Hypothesis semBindSize :
+  forall A B (g : G A) (f : A -> G B) (size : nat),
+    semGenSize (bindGen g f) size <-->
+    \bigcup_(a in semGenSize g size) semGenSize (f a) size.
 
-   Hypothesis semBindSize :
-     forall A B (g : G A) (f : A -> G B) (size : nat),
-       semGenSize (bindGen g f) size <-->
-       fun b => exists a, (semGenSize g size) a /\
-                          (semGenSize (f a) size) b.
+Hypothesis monad_leftid : 
+  forall {A B : Type} (a: A) (f : A -> G B),
+    semGen (bindGen (returnGen a) f) <--> semGen (f a).
+Hypothesis monad_rightid : 
+  forall {A : Type} (g : G A),
+    semGen (bindGen g returnGen) <--> semGen g.
+Hypothesis monad_assoc: 
+  forall {A B C : Type} (ga : G A) (fb : A -> G B) (fc : B -> G C),
+    semGen (bindGen (bindGen ga fb) fc) <--> 
+    semGen (bindGen ga (fun a => bindGen (fb a) fc)).
 
-   Hypothesis monad_leftid : 
-     forall {A B : Type} (a: A) (f : A -> G B),
-       semGen (bindGen (returnGen a) f) <--> semGen (f a).
-   Hypothesis monad_rightid : 
-     forall {A : Type} (g : G A),
-       semGen (bindGen g (fun a => returnGen a)) <--> semGen g.
-   Hypothesis monad_assoc: 
-     forall {A B C : Type} (ga : G A) (fb : A -> G B) (fc : B -> G C),
-       semGen (bindGen (bindGen ga fb) fc) <--> 
-       semGen (bindGen ga (fun a =>  bindGen (fb a) fc)).
+Hypothesis semFmap :
+  forall A B (f : A -> B) (g : G A),
+    semGen (fmap f g) <--> f @: semGen g.
+Hypothesis semFmapSize :
+  forall A B (f : A -> B) (g : G A) (size : nat),
+    semGenSize (fmap f g) size <--> f @: semGenSize g size.
 
-   Hypothesis semFmap :
-     forall A B (f : A -> B) (g : G A),
-       semGen (fmap f g) <-->
-       (fun b => exists a, (semGen g) a /\ b = f a).
-   Hypothesis semFmapSize :
-     forall A B (f : A -> B) (g : G A) (size : nat),
-       semGenSize (fmap f g) size <-->
-       (fun b => exists a, (semGenSize g size) a /\ b = f a).
+Hypothesis semChoose :
+  forall A `{Random A} a1 a2,
+    semGen (choose (a1,a2)) <-->
+    [set a | Random.leq a1 a /\ Random.leq a a2].
 
-   Hypothesis semChoose :
-     forall A `{Random A} a1 a2,
-       semGen (choose (a1,a2)) <-->
-       (fun a => Random.leq a1 a /\ Random.leq a a2).
-   Hypothesis semChooseSize :
-     forall A `{Random A} a1 a2 (size : nat),
-       semGenSize (choose (a1,a2)) size <-->
-       (fun a => Random.leq a1 a /\ Random.leq a a2).
+Hypothesis semChooseSize :
+  forall A `{Random A} a1 a2 (size : nat),
+    semGenSize (choose (a1,a2)) size <-->
+    [set a | Random.leq a1 a /\ Random.leq a a2].
 
-   Hypothesis semSized :
-     forall A (f : nat -> G A),
-       semGen (sized f) <--> (fun a => exists s, semGenSize (f s) s a).
-   Hypothesis semSizedSize :
-     forall A (f : nat -> G A) s,
-       semGenSize (sized f) s <--> (fun a => semGenSize (f s) s a).
+Hypothesis semSized :
+  forall A (f : nat -> G A),
+    semGen (sized f) <--> \bigcup_s semGenSize (f s) s.
+Hypothesis semSizedSize :
+  forall A (f : nat -> G A) s,
+    semGenSize (sized f) s <--> semGenSize (f s) s.
 
-   Hypothesis semResize :
-     forall A (n : nat) (g : G A),
-       semGen (resize n g) <--> semGenSize g n .
+Hypothesis semResize :
+  forall A (n : nat) (g : G A),
+    semGen (resize n g) <--> semGenSize g n.
 
-   (* TODO: We need completeness as well - this is not exact *)
-   Hypothesis semSuchThatMaybe_sound:
-     forall A (g : G A) (f : A -> bool),
-       semGen (suchThatMaybe g f) --->
-       (fun o => o = None \/
-                 (exists y, o = Some y /\ semGen g y /\ f y)).
+(* TODO: We need completeness as well - this is not exact *)
+Hypothesis semSuchThatMaybe_sound:
+  forall A (g : G A) (f : A -> bool),
+    semGen (suchThatMaybe g f) \subset
+    None |: some @: (semGen g :&: f).
 
-   (* This (very concrete) spec is needed to prove shrinking *)
-   Hypothesis semPromote :
-     forall A (m : Rose (G A)),
-       semGen (promote m) <-->
-       fun (t : (Rose A)) =>
-         exists seed size,
-          (fmapRose (fun (g : G A) => run g seed size) m) = t.
-   Hypothesis semPromoteSize :
-     forall (A : Type) (m : Rose (G A)) n,
-       semGenSize (promote m) n <-->
-       (fun t : Rose A =>
-          exists (seed : RandomSeed),
-            fmapRose (fun g : G A => run g seed n) m = t).
+(* This (very concrete) spec is needed to prove shrinking *)
+Hypothesis semPromote : forall A (m : Rose (G A)),
+  semGen (promote m) <-->
+  codom2 (fun size seed => fmapRose (fun g => run g size seed) m).
 
-   (* Those are too concrete, but I need them to prove shrinking.
-      Does this reveal a weakness in our framework?
-      Should we try to get rid of this?
-      This is expected since the spec of promote is too concrete. *)
+Hypothesis semPromoteSize :
+  forall (A : Type) (m : Rose (G A)) n,
+    semGenSize (promote m) n <-->
+    (fun t : Rose A =>
+       exists (seed : RandomSeed),
+         fmapRose (fun g : G A => run g n seed) m = t).
 
-   Hypothesis runFmap :
-     forall (A B : Type) (f : A -> B) (g : G A) seed size b,
-       run (fmap f g) seed size = b  <->
-       (exists a : A, run g seed size = a /\ b = f a).
-   Hypothesis runPromote :
-     forall A (m : Rose (G A)) seed size o,
-       run (promote m) seed size = o <->
-       (fmapRose (fun (g : G A) => run g seed size) m) = o.
+(* Those are too concrete, but I need them to prove shrinking.
+   Does this reveal a weakness in our framework?
+   Should we try to get rid of this?
+   This is expected since the spec of promote is too concrete. *)
+
+Hypothesis runFmap : forall (A B : Type) (f : A -> B) (g : G A) seed size,
+  run (fmap f g) seed size = f (run g seed size).
+  
+Hypothesis runPromote : forall A (m : Rose (G A)) seed size,
+  run (promote m) seed size = fmapRose (fun (g : G A) => run g seed size) m.
 
 End GenLowInterface.
 
 Module GenLow : GenLowInterface.
 
-   Inductive GenType (A : Type) : Type :=
-   | MkGen : (RandomSeed -> nat -> A) -> GenType A.
+Inductive GenType (A : Type) : Type :=
+| MkGen : (nat -> RandomSeed  -> A) -> GenType A.
 
-   Definition G := GenType.
+Definition G := GenType.
 
-   Definition run {A : Type} (g : G A) : RandomSeed -> nat -> A :=
-     match g with MkGen f => f end.
+Definition run {A : Type} (g : G A) : nat -> RandomSeed -> A :=
+  match g with MkGen f => f end.
 
-   Definition returnGen {A : Type} (x : A) : G A :=
-     MkGen (fun _ _ => x).
+Definition returnGen {A : Type} (x : A) : G A :=
+  MkGen (fun _ _ => x).
 
-   Definition bindGen {A B : Type} (g : G A) (k : A -> G B) : G B :=
-     MkGen (fun r n =>
-              let (r1,r2) := randomSplit r in
-               run (k (run g r1 n)) r2 n).
+Definition bindGen {A B : Type} (g : G A) (k : A -> G B) : G B :=
+  MkGen (fun n r =>
+           let (r1,r2) := randomSplit r in
+            run (k (run g n r1)) n r2).
 
-   Definition fmap {A B : Type} (f : A -> B) (g : G A) : G B :=
-     MkGen (fun r n => f ((run g) r n)).
+Definition fmap {A B : Type} (f : A -> B) (g : G A) : G B :=
+  MkGen (fun n r => f (run g n r)).
 
-   Definition sized {A : Type} (f : nat -> G A) : G A :=
-     MkGen (fun r n => run (f n) r n).
+Definition sized {A : Type} (f : nat -> G A) : G A :=
+  MkGen (fun n r => run (f n) n r).
 
-   Definition resize {A : Type} (n : nat) (g : G A) : G A :=
-     match g with
-       | MkGen m => MkGen (fun r _ => m r n)
-     end.
+Definition resize {A : Type} (n : nat) (g : G A) : G A :=
+  match g with
+    | MkGen m => MkGen (fun _ => m n)
+  end.
 
-   Definition promote {A : Type} (m : Rose (G A)) : G (Rose A) :=
-     MkGen (fun r n => fmapRose (fun g => run g r n) m).
+Definition promote {A : Type} (m : Rose (G A)) : G (Rose A) :=
+  MkGen (fun n r => fmapRose (fun g => run g n r) m).
 
-   (* ZP: Split suchThatMaybe into two different functions
-        to make a proof easier *)
-   Definition suchThatMaybeAux {A : Type} (g : G A) (p : A -> bool) :=
-     fix aux (k : nat) (n : nat) : G (option A) :=
-     match n with
-       | O => returnGen None
-       | S n' =>
-         bindGen (resize (2 * k + n) g) (fun x =>
-                                           if p x then returnGen (Some x)
-                                           else aux (S k) n')
-     end.
+(* ZP: Split suchThatMaybe into two different functions
+     to make a proof easier *)
+Definition suchThatMaybeAux {A : Type} (g : G A) (p : A -> bool) :=
+  fix aux (k : nat) (n : nat) : G (option A) :=
+  match n with
+    | O => returnGen None
+    | S n' =>
+      bindGen (resize (2 * k + n) g) (fun x =>
+                                        if p x then returnGen (Some x)
+                                        else aux (S k) n')
+  end.
 
-   Definition suchThatMaybe {A : Type} (g : G A) (p : A -> bool)
-   : G (option A) :=
-     sized (fun x => suchThatMaybeAux g p 0 (max 1 x)).
+Definition suchThatMaybe {A : Type} (g : G A) (p : A -> bool)
+: G (option A) :=
+  sized (fun x => suchThatMaybeAux g p 0 (max 1 x)).
 
-   Fixpoint rnds (rnd : RandomSeed) (n' : nat) : list RandomSeed :=
-     match n' with
-       | O => nil
-       | S n'' =>
-         let (rnd1, rnd2) := randomSplit rnd in
-         cons rnd1 (rnds rnd2 n'')
-     end.
+Fixpoint rnds (rnd : RandomSeed) (n' : nat) : list RandomSeed :=
+  match n' with
+    | O => nil
+    | S n'' =>
+      let (rnd1, rnd2) := randomSplit rnd in
+      cons rnd1 (rnds rnd2 n'')
+  end.
 
-   Fixpoint createRange (n : nat) (acc : list nat) : list nat :=
-     match n with
-       | O => List.rev (cons O acc)
-       | S n' => createRange n' (cons n acc)
-     end.
+Fixpoint createRange (n : nat) (acc : list nat) : list nat :=
+  match n with
+    | O => List.rev (cons O acc)
+    | S n' => createRange n' (cons n acc)
+  end.
 
-   Definition choose {A : Type} `{Random A} (range : A * A) : G A :=
-     MkGen (fun r _ => fst (randomR range r)).
+Definition choose {A : Type} `{Random A} (range : A * A) : G A :=
+  MkGen (fun _ r => fst (randomR range r)).
 
-   Definition sample (A : Type) (g : G A) : list A :=
-     match g with
-       | MkGen m =>
-         let rnd := mkRandomSeed 0 in
-         let l := List.combine (rnds rnd 20) (createRange 20 nil) in
-         List.map (fun (p : RandomSeed * nat) => let (r,n) := p in m r n) l
-     end.
+Definition sample (A : Type) (g : G A) : list A :=
+  match g with
+    | MkGen m =>
+      let rnd := mkRandomSeed 0 in
+      let l := List.combine (rnds rnd 20) (createRange 20 nil) in
+      List.map (fun (p : RandomSeed * nat) => let (r,n) := p in m n r) l
+  end.
 
 (* LL : Things that need to be in GenLow because of MkGen *)
 
-   Definition variant {A : Type} (p : SplitPath) (g : G A) : G A := 
-     match g with 
-       | MkGen f => MkGen (fun r n => f (varySeed p r) n)
-     end.
+Definition variant {A : Type} (p : SplitPath) (g : G A) : G A := 
+  match g with 
+    | MkGen f => MkGen (fun n r => f n (varySeed p r))
+  end.
 
-   Definition reallyUnsafeDelay {A : Type} : G (G A -> A) :=
-     MkGen (fun r n g => (match g with MkGen f => f r n end)).
-   
-   Definition reallyUnsafePromote {r A : Type} (m : r -> G A) : G (r -> A) :=
-       (bindGen reallyUnsafeDelay (fun eval => 
-        returnGen (fun r => eval (m r)))).
+Definition reallyUnsafeDelay {A : Type} : G (G A -> A) :=
+  MkGen (fun r n g => (match g with MkGen f => f r n end)).
+
+Definition reallyUnsafePromote {r A : Type} (m : r -> G A) : G (r -> A) :=
+    (bindGen reallyUnsafeDelay (fun eval => 
+     returnGen (fun r => eval (m r)))).
 (* End Things *)
 
-   (* Set of outcomes semantics definitions (repeated above) *)
-   Definition semGenSize {A : Type} (g : G A) (size : nat) : Ensemble A :=
-     fun a => exists seed, run g seed size = a.
-   Definition semGen {A : Type} (g : G A) : Ensemble A :=
-     fun a => exists size, semGenSize g size a.
+(* Set of outcomes semantics definitions (repeated above) *)
+Definition semGenSize {A : Type} (g : G A) (size : nat) : set A :=
+  codom (run g size).
+Definition semGen {A : Type} (g : G A) : set A :=
+  \bigcup_size semGenSize g size.
 
-   Lemma exists_const A P : inhabited A -> ((exists _ : A, P) <-> P).
-   Proof. by case=> ?; split=> //; case. Qed.
+Lemma semReturnSize A size (x : A) : semGenSize (returnGen x) size <--> [set x].
+Proof.
+by rewrite /semGenSize /= codom_const //; apply: randomSeed_inhabited.
+Qed.
 
-   Lemma semReturnSize A (x : A) size : semGenSize (returnGen x) size <--> eq x.
-   Proof.
-   rewrite /semGenSize /= /set_eq => ?; rewrite exists_const //.
-   exact: randomSeed_inhabited.
-   Qed.
+Lemma semReturn A (x : A) : semGen (returnGen x) <--> [set x].
+Proof.
+rewrite /semGen /semGenSize /= bigcup_const ?codom_const //.
+  exact: randomSeed_inhabited.
+by do 2! constructor.
+Qed.
 
-   Lemma semReturn A (x : A) : semGen (returnGen x) <--> eq x.
-   Proof.
-   rewrite /semGen /semGenSize /= => ?; rewrite !exists_const //.
-     exact: randomSeed_inhabited.
-   by do 2! constructor.
-   Qed.
+Lemma semBindSize A B (g : G A) (f : A -> G B) (size : nat) :
+  semGenSize (bindGen g f) size <-->
+  \bigcup_(a in semGenSize g size) semGenSize (f a) size.
+Proof.
+rewrite /semGenSize /bindGen /= bigcup_codom -curry_codom2l.
+by rewrite -[codom (prod_curry _)]imsetT -randomSplit_codom -codom_comp.
+Qed.
 
-   Lemma semBindSize : forall A B (g : G A) (f : A -> G B) (size : nat),
-                         semGenSize (bindGen g f) size <-->
-                                 fun b => exists a, (semGenSize g size) a /\
-                                                    (semGenSize (f a) size) b.
-   Proof.
-     move => A B [g] f size b. rewrite /semGenSize /bindGen => /=. split.
-     - case => [seed H]. move : H.
-       case (randomSplit seed) => [seed1 seed2] H.
-       exists (g seed1 size). split; eexists. reflexivity.
-       rewrite <- H. case (f (g seed1 size)). reflexivity.
-     - move => [a [[seed1 H1] [seed2 H2]]].
-       case (randomSplitAssumption seed1 seed2) => [seed Hseed].
-       exists seed. rewrite Hseed. rewrite H1. move : H2. by case (f a).
-   Qed.
+Lemma semFmapSize A B (f : A -> B) (g : G A) (size : nat) :
+  semGenSize (fmap f g) size <--> f @: semGenSize g size.
+Proof. by rewrite /fmap /semGenSize /= codom_comp. Qed.
 
-   Lemma semFmapSize : forall A B (f : A -> B) (g : G A) (size : nat),
-                         semGenSize (fmap f g) size <-->
-                                 (fun b => exists a, (semGenSize g size) a /\ b = f a).
-   Proof.
-     move => A B f [g] size b. rewrite /semGenSize /fmap => /=. split.
-     - move => [seed H]. exists (g seed size). by eauto.
-     - move => [a [[seed H1] H2]].
-       eexists. rewrite H2. rewrite <- H1. reflexivity.
-   Qed.
+Lemma monad_leftid A B (a : A) (f : A -> G B) :
+  semGen (bindGen (returnGen a) f) <--> semGen (f a).
+Proof.
+by apply: eq_bigcupr => size; rewrite semBindSize semReturnSize bigcup_set1.
+Qed.
 
-   Lemma monad_leftid : 
-     forall {A B : Type} (a: A) (f : A -> G B),
-       semGen (bindGen (returnGen a) f) <--> semGen (f a).
-   Proof. 
-     move => A B a f b. split => [[s /semBindSize [a' [/semReturnSize H1 H2]]] | [s H]]; subst.
-     - by exists s.
-     - exists s. apply semBindSize. exists a. split => //. by apply semReturnSize.
-   Qed.
+Lemma monad_rightid A (g : G A) : semGen (bindGen g returnGen) <--> semGen g.
+Proof.
+apply: eq_bigcupr => size; rewrite semBindSize.
+by rewrite (eq_bigcupr _ (semReturnSize size)) /semGenSize bigcup_codom codomE.
+Qed.
 
-   Lemma monad_rightid : 
-     forall {A : Type} (g : G A),
-       semGen (bindGen g (fun a => returnGen a)) <--> semGen g.
-     Proof.
-       move => A g a. split => [[s /semBindSize [a' [H1 /semReturnSize H2]]] 
-                               | [s H]]; subst.
-       - by exists s.
-       - exists s. apply semBindSize. exists a. split => //. by apply semReturnSize.
-     Qed.
-   
-   Lemma monad_assoc: 
-     forall {A B C : Type} (ga : G A) (fb : A -> G B) (fc : B -> G C),
-       semGen (bindGen (bindGen ga fb) fc) <--> 
-       semGen (bindGen ga (fun a =>  bindGen (fb a) fc)).
-   Proof.
-     move => A B C ga fb fc c. split => [[s /semBindSize [b [/semBindSize [a' [H1 H2]] H3]]] 
-                                        |[s /semBindSize [a' [H1 /semBindSize [b [H2 H3]]]]]];
-     exists s; by repeat (apply semBindSize; eexists; split; try eassumption).
-   Qed.
+Lemma monad_assoc A B C (ga : G A) (fb : A -> G B) (fc : B -> G C) :
+  semGen (bindGen (bindGen ga fb) fc) <--> 
+  semGen (bindGen ga (fun a => bindGen (fb a) fc)).
+Proof.
+(* Why can't we iterate here? *)
+apply eq_bigcupr => ?; rewrite !semBindSize ?bigcup_flatten.
+by apply eq_bigcupr => ?; rewrite !semBindSize ?bigcup_flatten.
+Qed.
 
-   (* TODO: This should just use semFMapSize *)
-   Lemma semFmap : forall A B (f : A -> B) (g : G A),
-                     semGen (fmap f g) <-->
-                            (fun b => exists a, (semGen g) a /\ b = f a).
+Lemma semFmap A B (f : A -> B) (g : G A) :
+  semGen (fmap f g) <--> f @: semGen g.
+Proof.
+by rewrite imset_bigcup /semGen (eq_bigcupr _ (semFmapSize _ _)).
+Qed.
 
-   Proof.
-     move => A B f [g] b. rewrite /semGen /semGenSize /fmap => /=. split.
-     - move => [size [seed H]]. exists (g seed size). by eauto.
-     - move => [a [[size [seed H1]] H2]].
-       do 2 eexists. rewrite H2. rewrite <- H1. reflexivity.
-   Qed.
+Lemma semChooseSize A `{Random A} a1 a2 size :
+    semGenSize (choose (a1,a2)) size <-->
+    [set a | Random.leq a1 a /\ Random.leq a a2].
+Proof. by move=> x /=; rewrite randomRCorrect. Qed.
 
-   Lemma semChooseSize :
-     forall A `{Random A} a1 a2 s,
-       semGenSize (choose (a1,a2)) s <-->
-       (fun a => Random.leq a1 a /\ Random.leq a a2).
-   Proof.
-     move => A R a1 a2 a. rewrite /semGen /semGenSize. simpl. split.
-     - move => [seed H]. apply randomRCorrect. by exists seed.
-     - by move => /randomRCorrect H.
-   Qed.
+Lemma semChoose A `{Random A} a1 a2 :
+    semGen (choose (a1,a2)) <-->
+    [set a | Random.leq a1 a /\ Random.leq a a2].
+Proof.
+rewrite /semGen (eq_bigcupr _ (semChooseSize _ _)) bigcup_const //.
+by do 2! constructor.
+Qed.
 
-   Lemma semChoose :
-     forall A `{Random A} a1 a2,
-       semGen (choose (a1,a2)) <-->
-       (fun a => Random.leq a1 a /\ Random.leq a a2).
-   Proof.
-     move => A R a1 a2 a. rewrite /semGen /semGenSize. simpl. split.
-     - by move => [_ /randomRCorrect H].
-     - move => /randomRCorrect H. by exists 0.
-   Qed.
+Lemma semSized A (f : nat -> G A) :
+  semGen (sized f) <--> \bigcup_n semGenSize (f n) n.
+Proof. by []. Qed.
 
+Lemma semSizedSize A (f : nat -> G A) s :
+    semGenSize (sized f) s <--> semGenSize (f s) s.
+Proof. by []. Qed.
 
-   Lemma semSized A (f : nat -> G A) :
-       semGen (sized f) <--> (fun a => exists n, semGenSize (f n) n a).
-   Proof. by []. Qed.
+Lemma semResize A n (g : G A) : semGen (resize n g) <--> semGenSize g n .
+Proof.
+by case: g => g; rewrite /semGen /semGenSize /= bigcup_const.
+Qed.
 
-   Lemma semSizedSize A (f : nat -> G A) s :
-       semGenSize (sized f) s <--> semGenSize (f s) s.
-   Proof. by []. Qed.
+Lemma semGenSuchThatMaybeAux_sound {A} : forall g p k n (a : A) size seed,
+  run (suchThatMaybeAux g p k n) size seed = Some a ->
+  a \in semGen g :&: p.
+Proof.
+case=> g p k n; elim: n k =>  [//=| n IHn] k a size seed /=.
+case: (randomSplit seed) => r1 r2; case: ifP=> [/= ? [<-]|_]; last exact: IHn.
+by split=> //; exists (2 * k + n.+1); split=> //; exists r1.
+Qed.
 
-   Lemma semResize :
-     forall A (n : nat) (g : G A), semGen (resize n g) <--> semGenSize g n .
-   Proof.
-     move => A n [g] a. rewrite /semGen /semGenSize /resize => /=. split.
-     - move => [_ [seed H]]. by eauto.
-     - move => [seed H]. exists 0. by eauto.
-   Qed.
+(* Not an exact spec !!! *)
+Lemma semSuchThatMaybe_sound A (g : G A) (f : A -> bool) :
+  semGen (suchThatMaybe g f) \subset
+  None |: some @: (semGen g :&: f).
+Proof.
+case=> [a [size [_ [x run_x]]] | ]; last by left.
+by right; exists a; split=> //; apply: (semGenSuchThatMaybeAux_sound run_x).
+Qed.
 
-   Lemma semGenSuchThatMaybeAux_sound:
-     forall {A} g p k n (a : A) seed size,
-       run (suchThatMaybeAux g p k n) seed size = Some a ->
-       (exists size seed, run g seed size = a) /\ p a.
-   Proof.
-     move=> /= A g p k n. elim : n k =>  [//=| n IHn] k a seed size H.
-     simpl in *. unfold run, bindGen in H.
-     remember (resize (2 * k + n.+1) g) as g'.
-     case: g' H Heqg'=> /= g' H Heqg'.
-     case: (randomSplit seed) H Heqg'=> /= r1 r2 H Heqg'.
-     remember (p (g' r1 size)) as b.
-     case: b H Heqb => /= H Heqb. inversion H; subst.
-     rewrite /resize in Heqg'.
-     destruct g as [g]. inversion Heqg'; subst.
-     split =>  //=. by eexists; eexists.
-     eapply (IHn k.+1 a r2 size). rewrite -H.
-       by destruct (suchThatMaybeAux g p k.+1 n).
-   Qed.
+Lemma semPromote A (m : Rose (G A)) :
+  semGen (promote m) <-->
+  codom2 (fun size seed => fmapRose (fun g => run g size seed) m).
+Proof. by rewrite /codom2 curry_codom2l. Qed.
 
-   (* Not an exact spec !!! *)
-   Lemma semSuchThatMaybe_sound :
-     forall A (g : G A) (f : A -> bool),
-       semGen (suchThatMaybe g f) --->
-       (fun o => o = None \/
-                 (exists y, o = Some y /\ semGen g y /\ f y)).
-   Proof.
-     move => A g f a. rewrite /semGen /semGenSize.
-     - case : a => [a|] [n [s H]]; last by left. right.
-       eexists; split=> //=.
-                          remember (match n with
-                                      | 0 => 1
-                                      | m'.+1 => m'.+1
-                                    end) as n'.
-       apply (semGenSuchThatMaybeAux_sound g f 0 n' s n). rewrite -H /= -Heqn'.
-         by destruct (suchThatMaybeAux g f 0 n').
-   Qed.
+Lemma semPromoteSize (A : Type) (m : Rose (G A)) n :
+  semGenSize (promote m) n <-->
+  codom (fun seed => fmapRose (fun g => run g n seed) m).
+Proof. by []. Qed.
 
-   Lemma semPromote :
-     forall A (m : Rose (G A)),
-       semGen (promote m) <-->
-       fun (t : (Rose A)) =>
-         exists seed size,
-           (fmapRose (fun (g : G A) => run g seed size) m) = t.
-   Proof.
-     move => A rg r. split;
-     move => [size [seed H]]; exists seed; exists size=> //=.
-   Qed.
+(* Those are too concrete, but I need them to prove shrinking.
+   Does this reveal a weakness in our framework?
+   Should we try to get rid of this?
+   This is expected since the spec of promote is too concrete.
+ *)
+Lemma runFmap (A B : Type) (f : A -> B) (g : G A) seed size :
+  run (fmap f g) seed size = f (run g seed size).
+Proof. by []. Qed.
 
-   Lemma semPromoteSize
-   : forall (A : Type) (m : Rose (G A)) n,
-       semGenSize (promote m) n <-->
-               (fun t : Rose A =>
-                  exists (seed : RandomSeed),
-                    fmapRose (fun g : G A => run g seed n) m = t).
-   Proof.
-     move => A rg r. split;
-     move => [seed H]; exists seed=> //=.
-   Qed.
-
-   (* Those are too concrete, but I need them to prove shrinking.
-      Does this reveal a weakness in our framework?
-      Should we try to get rid of this?
-      This is expected since the spec of promote is too concrete.
-    *)
-   Lemma runFmap :
-     forall (A B : Type) (f : A -> B) (g : G A) seed size b,
-       run (fmap f g) seed size = b  <->
-       (exists a : A, run g seed size = a /\ b = f a).
-   Proof.
-     move => A B f g seed size b'. split => /=.
-     - move => <-. eexists; split => //.
-     - by move => [a [Heq1 Heq2]]; subst.
-   Qed.
-
-   Lemma runPromote :
-     forall A (m : Rose (G A)) seed size o,
-       run (promote m) seed size = o <->
-       (fmapRose (fun (g : G A) => run g seed size) m) = o.
-   Proof.
-     move => A g x. split => //=.
-   Qed.
+Lemma runPromote A (m : Rose (G A)) seed size :
+  run (promote m) seed size = fmapRose (fun (g : G A) => run g seed size) m.
+Proof. by []. Qed.
 
 End GenLow.
