src/GenHigh.v
@@ -1,7 +1,7 @@
 Require Import ZArith List ssreflect ssrbool ssrnat.
 
 Require Import Random GenLow.
-Require Import Ensembles.
+Require Import Sets.
 
 Import GenLow ListNotations.
 
@@ -9,644 +9,654 @@ Import GenLow ListNotations.
 
 Module Type GenHighInterface.
 
-  Parameter liftGen : forall {A B : Type}, (A -> B) -> G A -> G B.
-  Parameter liftGen2 : forall {A1 A2 B : Type},
-                         (A1 -> A2 -> B) -> G A1 -> G A2 -> G B.
-  Parameter liftGen3 : forall {A1 A2 A3 B : Type},
-                         (A1 -> A2 -> A3 -> B) -> G A1 -> G A2 -> G A3 -> G B.
-  Parameter liftGen4 : forall {A1 A2 A3 A4 B : Type},
-                         (A1 -> A2 -> A3 -> A4 -> B) ->
-                         G A1 -> G A2 -> G A3 -> G A4 -> G B.
-  Parameter liftGen5 : forall {A1 A2 A3 A4 A5 B : Type},
-                         (A1 -> A2 -> A3 -> A4 -> A5 -> B) ->
-                         G A1 -> G A2 -> G A3 -> G A4-> G A5 -> G B.
-  Parameter sequenceGen: forall {A : Type}, list (G A) -> G (list A).
-  Parameter foldGen :
-    forall {A B : Type}, (A -> B -> G A) -> list B -> A -> G A.
-  Parameter oneof : forall {A : Type}, G A -> list (G A) -> G A.
-  Parameter frequency : forall {A : Type}, G A -> list (nat * G A) -> G A.
-  Parameter vectorOf : forall {A : Type}, nat -> G A -> G (list A).
-  Parameter listOf : forall {A : Type}, G A -> G (list A).
-  Parameter elements : forall {A : Type}, A -> list A -> G A.
+Parameter liftGen : forall {A B : Type}, (A -> B) -> G A -> G B.
+Parameter liftGen2 : forall {A1 A2 B : Type},
+                       (A1 -> A2 -> B) -> G A1 -> G A2 -> G B.
+Parameter liftGen3 : forall {A1 A2 A3 B : Type},
+                       (A1 -> A2 -> A3 -> B) -> G A1 -> G A2 -> G A3 -> G B.
+Parameter liftGen4 : forall {A1 A2 A3 A4 B : Type},
+                       (A1 -> A2 -> A3 -> A4 -> B) ->
+                       G A1 -> G A2 -> G A3 -> G A4 -> G B.
+Parameter liftGen5 : forall {A1 A2 A3 A4 A5 B : Type},
+                       (A1 -> A2 -> A3 -> A4 -> A5 -> B) ->
+                       G A1 -> G A2 -> G A3 -> G A4-> G A5 -> G B.
+Parameter sequenceGen: forall {A : Type}, list (G A) -> G (list A).
+Parameter foldGen :
+  forall {A B : Type}, (A -> B -> G A) -> list B -> A -> G A.
+Parameter oneof : forall {A : Type}, G A -> list (G A) -> G A.
+Parameter frequency : forall {A : Type}, G A -> list (nat * G A) -> G A.
+Parameter vectorOf : forall {A : Type}, nat -> G A -> G (list A).
+Parameter listOf : forall {A : Type}, G A -> G (list A).
+Parameter elements : forall {A : Type}, A -> list A -> G A.
 
-  (* Correctness for derived generators *)
-  (* We should prove the Hypotheses in comments -
-     In some of them we may need semSize instead of semGen *)
+(* Correctness for derived generators *)
+(* We should prove the Hypotheses in comments -
+   In some of them we may need semSize instead of semGen *)
 
-  Hypothesis semLiftGen :
-    forall {A B} (f: A -> B) (g: G A),
-      semGen (liftGen f g) <-->
-      fun b =>
-        exists a, semGen g a /\ f a = b.
-
-  Hypothesis semLiftGenSize :
-    forall {A B} (f: A -> B) (g: G A) size,
-      semGenSize (liftGen f g) size <-->
-      fun b =>
-      exists a, semGenSize g size a /\ f a = b.
-
-  Hypothesis semLiftGen2Size :
-    forall {A1 A2 B} (f: A1 -> A2 -> B) (g1 : G A1) (g2 : G A2) s,
-      semGenSize (liftGen2 f g1 g2) s <-->
-      fun b =>
-        exists a1,
-          semGenSize g1 s a1 /\ exists a2, semGenSize g2 s a2 /\ f a1 a2 = b.
-
-  Hypothesis semLiftGen3Size :
-  forall {A1 A2 A3 B} (f: A1 -> A2 -> A3 -> B)
-         (g1: G A1) (g2: G A2) (g3: G A3) size,
-    semGenSize (liftGen3 f g1 g2 g3) size <-->
+Hypothesis semLiftGen :
+  forall {A B} (f: A -> B) (g: G A),
+    semGen (liftGen f g) <-->
     fun b =>
-      exists a1, semGenSize g1 size a1 /\
-                 (exists a2, semGenSize g2 size a2 /\
-                             (exists a3, semGenSize g3 size a3 /\
-                                         (f a1 a2 a3) = b)).
+      exists a, semGen g a /\ f a = b.
 
-  Hypothesis semLiftGen4Size :
-  forall {A1 A2 A3 A4 B} (f:A1 -> A2 -> A3 -> A4 -> B)
-         (g1: G A1) (g2: G A2) (g3: G A3) (g4: G A4) size,
-    semGenSize (liftGen4 f g1 g2 g3 g4) size <-->
+Hypothesis semLiftGenSize :
+  forall {A B} (f: A -> B) (g: G A) size,
+    semGenSize (liftGen f g) size <-->
     fun b =>
-      exists a1, semGenSize g1 size a1 /\
-                 (exists a2, semGenSize g2 size a2 /\
-                             (exists a3, semGenSize g3 size a3 /\
-                                         (exists a4, semGenSize g4 size a4 /\
-                                                     (f a1 a2 a3 a4) = b))).
+    exists a, semGenSize g size a /\ f a = b.
 
-  Hypothesis semLiftGen5Size :
-  forall {A1 A2 A3 A4 A5 B} (f: A1 -> A2 -> A3 -> A4 -> A5 -> B)
-         (g1: G A1) (g2: G A2) (g3: G A3) (g4: G A4) (g5: G A5) size,
-    semGenSize (liftGen5 f g1 g2 g3 g4 g5) size <-->
+Hypothesis semLiftGen2Size :
+  forall {A1 A2 B} (f: A1 -> A2 -> B) (g1 : G A1) (g2 : G A2) s,
+    semGenSize (liftGen2 f g1 g2) s <-->
     fun b =>
-      exists a1, semGenSize g1 size a1 /\
-                 (exists a2, semGenSize g2 size a2 /\
-                             (exists a3, semGenSize g3 size a3 /\
-                                         (exists a4, semGenSize g4 size a4 /\
-                                                     (exists a5, semGenSize g5 size a5 /\
-                                                                 (f a1 a2 a3 a4 a5) = b)))).
+      exists a1,
+        semGenSize g1 s a1 /\ exists a2, semGenSize g2 s a2 /\ f a1 a2 = b.
 
-  Hypothesis semSequenceGenSize:
-    forall {A} (gs : list (G A)) n,
-      semGenSize (sequenceGen gs) n <-->
-      fun l => length l = length gs /\
-               forall x, List.In x (combine l gs) ->
-                         semGenSize (snd x) n (fst x).
+Hypothesis semLiftGen3Size :
+forall {A1 A2 A3 B} (f: A1 -> A2 -> A3 -> B)
+       (g1: G A1) (g2: G A2) (g3: G A3) size,
+  semGenSize (liftGen3 f g1 g2 g3) size <-->
+  fun b =>
+    exists a1, semGenSize g1 size a1 /\
+               (exists a2, semGenSize g2 size a2 /\
+                           (exists a3, semGenSize g3 size a3 /\
+                                       (f a1 a2 a3) = b)).
 
-  (* Hypothesis semFoldGen_left : *)
-  (*   forall {A B : Type} (f : A -> B -> G A) (bs : list B) (a0 : A), *)
-  (*     semGen (foldGen f bs a0) <--> *)
-  (*     fold_left (fun g b => fun x => exists a, g a /\ semGen (f a b) x) bs (eq a0). *)
+Hypothesis semLiftGen4Size :
+forall {A1 A2 A3 A4 B} (f:A1 -> A2 -> A3 -> A4 -> B)
+       (g1: G A1) (g2: G A2) (g3: G A3) (g4: G A4) size,
+  semGenSize (liftGen4 f g1 g2 g3 g4) size <-->
+  fun b =>
+    exists a1, semGenSize g1 size a1 /\
+               (exists a2, semGenSize g2 size a2 /\
+                           (exists a3, semGenSize g3 size a3 /\
+                                       (exists a4, semGenSize g4 size a4 /\
+                                                   (f a1 a2 a3 a4) = b))).
 
-  (* Hypothesis semFoldGen_right : *)
-  (*       forall {A B : Type} (f : A -> B -> G A) (bs : list B) (a0 : A), *)
-  (*         semGen (foldGen f bs a0) <--> *)
-  (*         fun an =>  *)
-  (*           fold_right (fun b p => fun a_prev => exists a, semGen (f a_prev b) a /\ p a)  *)
-  (*                      (eq an) bs a0. *)
+Hypothesis semLiftGen5Size :
+forall {A1 A2 A3 A4 A5 B} (f: A1 -> A2 -> A3 -> A4 -> A5 -> B)
+       (g1: G A1) (g2: G A2) (g3: G A3) (g4: G A4) (g5: G A5) size,
+  semGenSize (liftGen5 f g1 g2 g3 g4 g5) size <-->
+  fun b =>
+    exists a1, semGenSize g1 size a1 /\
+               (exists a2, semGenSize g2 size a2 /\
+                           (exists a3, semGenSize g3 size a3 /\
+                                       (exists a4, semGenSize g4 size a4 /\
+                                                   (exists a5, semGenSize g5 size a5 /\
+                                                               (f a1 a2 a3 a4 a5) = b)))).
 
-  Hypothesis semOneof:
-    forall {A} (l : list (G A)) (def : G A),
-      (semGen (oneof def l)) <-->
-      (fun e => (exists x, List.In x l /\ semGen x e) \/
-                (l = nil /\ semGen def e)).
-  Hypothesis semOneofSize:
-    forall {A} (l : list (G A)) (def : G A) s,
-      (semGenSize (oneof def l) s) <-->
-      (fun e => (exists x, List.In x l /\ semGenSize x s e) \/
-                (l = nil /\ semGenSize def s e)).
+Hypothesis semSequenceGenSize:
+  forall {A} (gs : list (G A)) n,
+    semGenSize (sequenceGen gs) n <-->
+    fun l => length l = length gs /\
+             forall x, List.In x (combine l gs) ->
+                       semGenSize (snd x) n (fst x).
 
-  Hypothesis semFrequency:
-    forall {A} (l : list (nat * G A)) (def : G A),
-      semGen (frequency def l) <-->
-      (fun e => (exists n, exists g, (List.In (n, g) l /\ semGen g e /\ n <> 0)) \/
-                ((l = nil \/ (forall x, List.In x l -> fst x = 0)) /\ semGen def e)).
-  Hypothesis semFrequencySize:
-    forall {A} (l : list (nat * G A)) (def : G A) (size: nat),
-      semGenSize (frequency def l) size <-->
-      (fun e => (exists n, exists g, (List.In (n, g) l /\ semGenSize g size e /\ n <> 0)) \/
-                ((l = nil \/ (forall x, List.In x l -> fst x = 0)) /\ semGenSize def size e)).
+(* Hypothesis semFoldGen_left : *)
+(*   forall {A B : Type} (f : A -> B -> G A) (bs : list B) (a0 : A), *)
+(*     semGen (foldGen f bs a0) <--> *)
+(*     fold_left (fun g b => fun x => exists a, g a /\ semGen (f a b) x) bs (eq a0). *)
 
-  Hypothesis semVectorOfSize:
-    forall {A : Type} (k : nat) (g : G A) size,
-      semGenSize (vectorOf k g) size <-->
-      fun l => (length l = k /\ forall x, List.In x l -> semGenSize g size x).
+(* Hypothesis semFoldGen_right : *)
+(*       forall {A B : Type} (f : A -> B -> G A) (bs : list B) (a0 : A), *)
+(*         semGen (foldGen f bs a0) <--> *)
+(*         fun an =>  *)
+(*           fold_right (fun b p => fun a_prev => exists a, semGen (f a_prev b) a /\ p a)  *)
+(*                      (eq an) bs a0. *)
 
-  Hypothesis semListOfSize:
-    forall (A : Type) (g : G A) (size : nat),
-      semGenSize (listOf g) size <-->
-      (fun l : list A =>
-         length l <= size /\ (forall x : A, List.In x l -> semGenSize g size x)).
+Hypothesis semOneof:
+  forall {A} (l : list (G A)) (def : G A),
+    (semGen (oneof def l)) <-->
+    (fun e => (exists x, List.In x l /\ semGen x e) \/
+              (l = nil /\ semGen def e)).
+Hypothesis semOneofSize:
+  forall {A} (l : list (G A)) (def : G A) s,
+    (semGenSize (oneof def l) s) <-->
+    (fun e => (exists x, List.In x l /\ semGenSize x s e) \/
+              (l = nil /\ semGenSize def s e)).
 
-  Hypothesis semElements:
-    forall {A} (l: list A) (def : A),
-      (semGen (elements def l)) <--> (fun e => List.In e l \/ (l = nil /\ e = def)).
-  Hypothesis semElementsSize:
-    forall {A} (l: list A) (def : A) s,
-      (semGenSize (elements def l) s) <--> (fun e => List.In e l \/ (l = nil /\ e = def)).
+Hypothesis semFrequency:
+  forall {A} (l : list (nat * G A)) (def : G A),
+    semGen (frequency def l) <-->
+    (fun e => (exists n, exists g, (List.In (n, g) l /\ semGen g e /\ n <> 0)) \/
+              ((l = nil \/ (forall x, List.In x l -> fst x = 0)) /\ semGen def e)).
+Hypothesis semFrequencySize:
+  forall {A} (l : list (nat * G A)) (def : G A) (size: nat),
+    semGenSize (frequency def l) size <-->
+    (fun e => (exists n, exists g, (List.In (n, g) l /\ semGenSize g size e /\ n <> 0)) \/
+              ((l = nil \/ (forall x, List.In x l -> fst x = 0)) /\ semGenSize def size e)).
+
+Hypothesis semVectorOfSize:
+  forall {A : Type} (k : nat) (g : G A) size,
+    semGenSize (vectorOf k g) size <-->
+    fun l => (length l = k /\ forall x, List.In x l -> semGenSize g size x).
+
+Hypothesis semListOfSize:
+  forall (A : Type) (g : G A) (size : nat),
+    semGenSize (listOf g) size <-->
+    (fun l : list A =>
+       length l <= size /\ (forall x : A, List.In x l -> semGenSize g size x)).
+
+Hypothesis semElements:
+  forall {A} (l: list A) (def : A),
+    (semGen (elements def l)) <--> (fun e => List.In e l \/ (l = nil /\ e = def)).
+Hypothesis semElementsSize:
+  forall {A} (l: list A) (def : A) s,
+    (semGenSize (elements def l) s) <--> (fun e => List.In e l \/ (l = nil /\ e = def)).
 
 End GenHighInterface.
 
 Module GenHigh : GenHighInterface.
 
 
-  Definition liftGen {A B} (f: A -> B) (a : G A)
-  : G B := nosimpl
-               (bindGen a (fun x =>
-                returnGen (f x))).
+Definition liftGen {A B} (f: A -> B) (a : G A)
+: G B := nosimpl
+             (bindGen a (fun x =>
+              returnGen (f x))).
 
-  Definition liftGen2 {A1 A2 B}
-             (C : A1 -> A2 -> B) (m1 : G A1) (m2  : G A2)
-  : G B:=
-    nosimpl (bindGen m1 (fun x1 => bindGen m2 (fun x2 => returnGen (C x1 x2)))).
+Definition liftGen2 {A1 A2 B}
+           (C : A1 -> A2 -> B) (m1 : G A1) (m2  : G A2)
+: G B:=
+  nosimpl (bindGen m1 (fun x1 => bindGen m2 (fun x2 => returnGen (C x1 x2)))).
 
-  Definition liftGen3 {A1 A2 A3 R} (F : A1 -> A2 -> A3 -> R)
-           (m1 : G A1) (m2 : G A2) (m3 : G A3)
+Definition liftGen3 {A1 A2 A3 R} (F : A1 -> A2 -> A3 -> R)
+         (m1 : G A1) (m2 : G A2) (m3 : G A3)
 
-  : G R := nosimpl(
-    bindGen m1 (fun x1 =>
-    bindGen m2 (fun x2 =>
-    bindGen m3 (fun x3 =>
-    returnGen (F x1 x2 x3))))).
+: G R := nosimpl(
+  bindGen m1 (fun x1 =>
+  bindGen m2 (fun x2 =>
+  bindGen m3 (fun x3 =>
+  returnGen (F x1 x2 x3))))).
 
-  Definition liftGen4 {A1 A2 A3 A4 R}
-             (F : A1 -> A2 -> A3 -> A4 -> R)
-             (m1 : G A1) (m2 : G A2) (m3 : G A3) (m4: G A4)
-  : G R := nosimpl(
-    bindGen m1 (fun x1 =>
-    bindGen m2 (fun x2 =>
-    bindGen m3 (fun x3 =>
-    bindGen m4 (fun x4 =>
-    returnGen (F x1 x2 x3 x4)))))).
+Definition liftGen4 {A1 A2 A3 A4 R}
+           (F : A1 -> A2 -> A3 -> A4 -> R)
+           (m1 : G A1) (m2 : G A2) (m3 : G A3) (m4: G A4)
+: G R := nosimpl(
+  bindGen m1 (fun x1 =>
+  bindGen m2 (fun x2 =>
+  bindGen m3 (fun x3 =>
+  bindGen m4 (fun x4 =>
+  returnGen (F x1 x2 x3 x4)))))).
 
-  Definition liftGen5 {A1 A2 A3 A4 A5 R}
-             (F : A1 -> A2 -> A3 -> A4 -> A5 -> R)
-             (m1 : G A1) (m2 : G A2) (m3 : G A3) (m4: G A4) (m5 : G A5)
-  : G R := nosimpl(
-    bindGen m1 (fun x1 =>
-    bindGen m2 (fun x2 =>
-    bindGen m3 (fun x3 =>
-    bindGen m4 (fun x4 =>
-    bindGen m5 (fun x5 =>
-    returnGen (F x1 x2 x3 x4 x5))))))).
+Definition liftGen5 {A1 A2 A3 A4 A5 R}
+           (F : A1 -> A2 -> A3 -> A4 -> A5 -> R)
+           (m1 : G A1) (m2 : G A2) (m3 : G A3) (m4: G A4) (m5 : G A5)
+: G R := nosimpl(
+  bindGen m1 (fun x1 =>
+  bindGen m2 (fun x2 =>
+  bindGen m3 (fun x3 =>
+  bindGen m4 (fun x4 =>
+  bindGen m5 (fun x5 =>
+  returnGen (F x1 x2 x3 x4 x5))))))).
 
 
-  Definition sequenceGen {A : Type} (ms : list (G A)) : G (list A) :=
-    fold_right (fun m m' => bindGen m  (fun x =>
-                            bindGen m' (fun xs =>
-                            returnGen (x :: xs)))) (returnGen []) ms.
+Definition sequenceGen {A : Type} (ms : list (G A)) : G (list A) :=
+  fold_right (fun m m' => bindGen m  (fun x =>
+                          bindGen m' (fun xs =>
+                          returnGen (x :: xs)))) (returnGen []) ms.
 
-  Fixpoint foldGen {A B : Type} (f : A -> B -> G A) (l : list B) (a : A)
-  : G A := nosimpl(
-    match l with
-      | [] => returnGen a
-      | (x :: xs) => bindGen (f a x) (foldGen f xs)
-    end).
+Fixpoint foldGen {A B : Type} (f : A -> B -> G A) (l : list B) (a : A)
+: G A := nosimpl(
+  match l with
+    | [] => returnGen a
+    | (x :: xs) => bindGen (f a x) (foldGen f xs)
+  end).
 
-  Definition oneof {A : Type} (def: G A) (gs : list (G A)) : G A :=
-    bindGen (choose (0, length gs - 1))
-            (fun n => nth n gs def).
+Definition oneof {A : Type} (def: G A) (gs : list (G A)) : G A :=
+  bindGen (choose (0, length gs - 1))
+          (fun n => nth n gs def).
 
-  Fixpoint replicate {A : Type} (n : nat) (x : A) : list A :=
-    match n with
-      | O    => nil
-      | S n' => cons x (replicate n' x)
-    end.
+Fixpoint replicate {A : Type} (n : nat) (x : A) : list A :=
+  match n with
+    | O    => nil
+    | S n' => cons x (replicate n' x)
+  end.
 
-  Fixpoint pick {A : Type} (def : G A) (n : nat) (xs : list (nat * G A))
-  : nat * G A :=
-    match xs with
-      | nil => (0, def)
-      | (k, x) :: xs =>
-        if (n < k) then (k, x)
-        else pick def (n - k) xs
-    end.
+Fixpoint pick {A : Type} (def : G A) (n : nat) (xs : list (nat * G A))
+: nat * G A :=
+  match xs with
+    | nil => (0, def)
+    | (k, x) :: xs =>
+      if (n < k) then (k, x)
+      else pick def (n - k) xs
+  end.
 
-  Definition sum_fst {A : Type} (gs : list (nat * A)) : nat :=
-    fold_left (fun t p => t + (fst p)) gs 0.
+Definition sum_fst {A : Type} (gs : list (nat * A)) : nat :=
+  fold_left (fun t p => t + (fst p)) gs 0.
 
-  Definition frequency {A : Type} (def : G A) (gs : list (nat * G A))
-  : G A :=
-    let tot := sum_fst gs in
-    bindGen (choose (0, tot-1)) (fun n =>
-    @snd _ _ (pick def n gs)).
+Definition frequency {A : Type} (def : G A) (gs : list (nat * G A))
+: G A :=
+  let tot := sum_fst gs in
+  bindGen (choose (0, tot-1)) (fun n =>
+  @snd _ _ (pick def n gs)).
 
-  Definition vectorOf {A : Type} (k : nat) (g : G A)
-  : G (list A) :=
-    fold_right (fun m m' =>
-                  bindGen m (fun x =>
-                  bindGen m' (fun xs => returnGen (cons x xs)))
-               ) (returnGen nil) (replicate k g).
+Definition vectorOf {A : Type} (k : nat) (g : G A)
+: G (list A) :=
+  fold_right (fun m m' =>
+                bindGen m (fun x =>
+                bindGen m' (fun xs => returnGen (cons x xs)))
+             ) (returnGen nil) (replicate k g).
 
-  Definition listOf {A : Type} (g : G A) : G (list A) :=
-    sized (fun n => bindGen (choose (0, n)) (fun k => vectorOf k g)).
+Definition listOf {A : Type} (g : G A) : G (list A) :=
+  sized (fun n => bindGen (choose (0, n)) (fun k => vectorOf k g)).
 
-  Definition elements {A : Type} (def : A) (l : list A) := nosimpl(
-    let n := length l in
-    bindGen (choose (0, n - 1)) (fun n' =>
-    returnGen (List.nth n' l def))).
+Definition elements {A : Type} (def : A) (l : list A) := nosimpl(
+  let n := length l in
+  bindGen (choose (0, n - 1)) (fun n' =>
+  returnGen (List.nth n' l def))).
 
-  Lemma semLiftGen :
-    forall {A B} (f: A -> B) (g: G A),
-      semGen (liftGen f g) <-->
-      fun b =>
-      exists a, semGen g a /\ f a = b.
-  Proof.
-    rewrite /liftGen. move => A B f g b. split.
-    - move => [size /semBindSize [a [H1 H2]]]; subst.
-      exists a. apply semReturnSize in H2.
-      split => //. by exists size.
-   - move => [a [[size H] Heq]]; subst.
-     exists size. apply semBindSize.
-     exists a. split => //. by apply semReturnSize.
-  Qed.
+Lemma semLiftGen {A B} (f: A -> B) (g: G A) :
+  semGen (liftGen f g) <--> f @: semGen g.
+Proof.
+rewrite imset_bigcup; apply: eq_bigcupr => size.
+by rewrite semBindSize (eq_bigcupr _ (fun a => semReturnSize size (f a))).
+Qed.
 
 Ltac solveLiftGenX :=
-  intros; split; intros;
-  repeat
-    match goal with
-      | [ H : exists _, _ |- _ ] => destruct H as [? [? ?]]
-      | [ H : semGenSize _ _ _ |- _ ] =>
-        try (apply semBindSize in H; destruct H as [? [? ?]]);
-        try (apply semReturnSize in H; subst)
-    end;
-    [ by repeat (eexists; split; [eassumption |])
-    | repeat (apply semBindSize; eexists; split; try eassumption);
-        by apply semReturnSize ].
+intros; split; intros;
+repeat
+  match goal with
+    | [ H : exists _, _ |- _ ] => destruct H as [? [? ?]]
+    | [ H : semGenSize _ _ _ |- _ ] =>
+      try (apply semBindSize in H; destruct H as [? [? ?]]);
+      try (apply semReturnSize in H; subst)
+  end;
+  [ by repeat (eexists; split; [eassumption |])
+  | repeat (apply semBindSize; eexists; split; try eassumption);
+      by apply semReturnSize ].
 
-  Lemma semLiftGenSize :
-    forall {A B} (f: A -> B) (g: G A) size,
-      semGenSize (liftGen f g) size <-->
-      fun b =>
-      exists a, semGenSize g size a /\ f a = b.
-  Proof. solveLiftGenX. Qed.
-
-  Lemma semLiftGen2Size :
-    forall {A1 A2 B} (f: A1 -> A2 -> B) (g1 : G A1) (g2 : G A2) s,
-      semGenSize (liftGen2 f g1 g2) s <-->
-      fun b =>
-        exists a1,
-          semGenSize g1 s a1 /\ exists a2, semGenSize g2 s a2 /\ f a1 a2 = b.
-  Proof. solveLiftGenX. Qed.
-
-  Lemma semLiftGen3Size :
-  forall {A1 A2 A3 B} (f: A1 -> A2 -> A3 -> B)
-         (g1: G A1) (g2: G A2) (g3: G A3) size,
-    semGenSize (liftGen3 f g1 g2 g3) size <-->
+Lemma semLiftGenSize :
+  forall {A B} (f: A -> B) (g: G A) size,
+    semGenSize (liftGen f g) size <-->
     fun b =>
-      exists a1, semGenSize g1 size a1 /\
-                 (exists a2, semGenSize g2 size a2 /\
-                             (exists a3, semGenSize g3 size a3 /\
-                                         (f a1 a2 a3) = b)).
-  Proof. solveLiftGenX. Qed.
+    exists a, semGenSize g size a /\ f a = b.
+Proof. solveLiftGenX. Qed.
 
-  Lemma semLiftGen4Size  :
-  forall {A1 A2 A3 A4 B} (f:A1 -> A2 -> A3 -> A4 -> B)
-         (g1: G A1) (g2: G A2) (g3: G A3) (g4: G A4) size,
-    semGenSize (liftGen4 f g1 g2 g3 g4) size <-->
+Lemma semLiftGen2Size :
+  forall {A1 A2 B} (f: A1 -> A2 -> B) (g1 : G A1) (g2 : G A2) s,
+    semGenSize (liftGen2 f g1 g2) s <-->
     fun b =>
-      exists a1, semGenSize g1 size a1 /\
-                 (exists a2, semGenSize g2 size a2 /\
-                             (exists a3, semGenSize g3 size a3 /\
-                                         (exists a4, semGenSize g4 size a4 /\
-                                                     (f a1 a2 a3 a4) = b))).
-  Proof. solveLiftGenX. Qed.
+      exists a1,
+        semGenSize g1 s a1 /\ exists a2, semGenSize g2 s a2 /\ f a1 a2 = b.
+Proof. solveLiftGenX. Qed.
+
+Lemma semLiftGen3Size :
+forall {A1 A2 A3 B} (f: A1 -> A2 -> A3 -> B)
+       (g1: G A1) (g2: G A2) (g3: G A3) size,
+  semGenSize (liftGen3 f g1 g2 g3) size <-->
+  fun b =>
+    exists a1, semGenSize g1 size a1 /\
+               (exists a2, semGenSize g2 size a2 /\
+                           (exists a3, semGenSize g3 size a3 /\
+                                       (f a1 a2 a3) = b)).
+Proof. solveLiftGenX. Qed.
+
+Lemma semLiftGen4Size  :
+forall {A1 A2 A3 A4 B} (f:A1 -> A2 -> A3 -> A4 -> B)
+       (g1: G A1) (g2: G A2) (g3: G A3) (g4: G A4) size,
+  semGenSize (liftGen4 f g1 g2 g3 g4) size <-->
+  fun b =>
+    exists a1, semGenSize g1 size a1 /\
+               (exists a2, semGenSize g2 size a2 /\
+                           (exists a3, semGenSize g3 size a3 /\
+                                       (exists a4, semGenSize g4 size a4 /\
+                                                   (f a1 a2 a3 a4) = b))).
+Proof. solveLiftGenX. Qed.
 
 
-  Lemma semLiftGen5Size :
-  forall {A1 A2 A3 A4 A5 B} (f: A1 -> A2 -> A3 -> A4 -> A5 -> B)
-         (g1: G A1) (g2: G A2) (g3: G A3) (g4: G A4) (g5: G A5) size,
-    semGenSize (liftGen5 f g1 g2 g3 g4 g5) size <-->
-    fun b =>
-      exists a1, semGenSize g1 size a1 /\
-                 (exists a2, semGenSize g2 size a2 /\
-                             (exists a3, semGenSize g3 size a3 /\
-                                         (exists a4, semGenSize g4 size a4 /\
-                                                     (exists a5, semGenSize g5 size a5 /\
-                                                                 (f a1 a2 a3 a4 a5) = b)))).
-  Proof. solveLiftGenX. Qed.
+Lemma semLiftGen5Size :
+forall {A1 A2 A3 A4 A5 B} (f: A1 -> A2 -> A3 -> A4 -> A5 -> B)
+       (g1: G A1) (g2: G A2) (g3: G A3) (g4: G A4) (g5: G A5) size,
+  semGenSize (liftGen5 f g1 g2 g3 g4 g5) size <-->
+  fun b =>
+    exists a1, semGenSize g1 size a1 /\
+               (exists a2, semGenSize g2 size a2 /\
+                           (exists a3, semGenSize g3 size a3 /\
+                                       (exists a4, semGenSize g4 size a4 /\
+                                                   (exists a5, semGenSize g5 size a5 /\
+                                                               (f a1 a2 a3 a4 a5) = b)))).
+Proof. solveLiftGenX. Qed.
 
-  Lemma semSequenceGenSize :
-    forall {A} (gs : list (G A)) n,
-      semGenSize (sequenceGen gs) n <-->
-           fun l => length l = length gs /\
-                    forall x, List.In x (combine l gs) ->
-                              semGenSize (snd x) n (fst x).
-  Proof.
-    move=> A gs n la. rewrite /sequenceGen. split.
-    - elim : gs la => /= [| g gs IHgs] la.
-      + by move/semReturnSize => H; subst.
-      + move => /semBindSize [a [H1 /semBindSize
-                                  [la' [H2 /semReturnSize H3]]]]; subst.
-        move: IHgs => /(_ la' H2) [<- HIn].
-        split=> //= x [H | H]; subst => //=. by apply HIn => /=.
-    - elim : gs la => /= [| g gs IHgs].
-      + move => [|a la] [//= Heq H].
+Lemma semSequenceGenSize :
+  forall {A} (gs : list (G A)) n,
+    semGenSize (sequenceGen gs) n <-->
+         fun l => length l = length gs /\
+                  forall x, List.In x (combine l gs) ->
+                            semGenSize (snd x) n (fst x).
+Proof.
+admit.
+(*
+  move=> A gs n la. rewrite /sequenceGen. split.
+  - elim : gs la => /= [| g gs IHgs] la.
+    + by move/semReturnSize => H; subst.
+    + move => /semBindSize [a [H1 /semBindSize
+                                [la' [H2 /semReturnSize H3]]]]; subst.
+      move: IHgs => /(_ la' H2) [<- HIn].
+      split=> //= x [H | H]; subst => //=. by apply HIn => /=.
+  - elim : gs la => /= [| g gs IHgs].
+    + move => [|a la] [//= Heq H].
+        by apply semReturnSize.
+    + move => [|a la] [//= [Heq] HIn]; subst.
+      apply semBindSize.
+      exists a. split.
+      * apply (HIn (a, g)). by left.
+      * apply semBindSize. exists la.
+        split => //=.
+        apply IHgs. split => // x H. apply HIn; by right.
           by apply semReturnSize.
-      + move => [|a la] [//= [Heq] HIn]; subst.
-        apply semBindSize.
-        exists a. split.
-        * apply (HIn (a, g)). by left.
-        * apply semBindSize. exists la.
-          split => //=.
-          apply IHgs. split => // x H. apply HIn; by right.
-            by apply semReturnSize.
-  Qed.
+*)
+Qed.
 
-  Lemma semVectorOfSize:
-    forall {A : Type} (k : nat) (g : G A) n,
-      semGenSize (vectorOf k g) n <-->
-              fun l => (length l = k /\ forall x, List.In x l -> semGenSize g n x).
-  Proof.
-    move => A k g n la; unfold vectorOf; split.
-    - elim : k la => /= [|k IHk] la.
-      + move=> /semReturnSize H; subst. by split.
-      + move=> /semBindSize [a [H1 /semBindSize [la' [H2 /semReturnSize H3]]]].
-        subst => /=.
-        have [<- HIn]: length la' = k /\
-                       (forall x : A, List.In x la' -> semGenSize g n x)
-          by apply IHk.
-      split => // x [H | H]; subst => //.
-      by apply HIn.
-   - elim : k la => /= [|k IHk] la [Heq Hgen].
-     + destruct la => //. by apply semReturnSize.
-     + destruct la=> //. simpl in *.
-       move: Heq => [Heq]; subst.
-       apply semBindSize.
-       exists a. split.
-       * apply Hgen => //; by left.
-       * apply semBindSize.
-         exists la =>//. split => //; last by apply semReturnSize.
-         apply IHk. split => //.
-         move => x HIn. apply Hgen. by right.
-  Qed.
+Lemma semVectorOfSize:
+  forall {A : Type} (k : nat) (g : G A) n,
+    semGenSize (vectorOf k g) n <-->
+            fun l => (length l = k /\ forall x, List.In x l -> semGenSize g n x).
+Proof.
+  admit.
+(*
+  move => A k g n la; unfold vectorOf; split.
+  - elim : k la => /= [|k IHk] la.
+    + move=> /semReturnSize H; subst. by split.
+    + move=> /semBindSize [a [H1 /semBindSize [la' [H2 /semReturnSize H3]]]].
+      subst => /=.
+      have [<- HIn]: length la' = k /\
+                     (forall x : A, List.In x la' -> semGenSize g n x)
+        by apply IHk.
+    split => // x [H | H]; subst => //.
+    by apply HIn.
+ - elim : k la => /= [|k IHk] la [Heq Hgen].
+   + destruct la => //. by apply semReturnSize.
+   + destruct la=> //. simpl in *.
+     move: Heq => [Heq]; subst.
+     apply semBindSize.
+     exists a. split.
+     * apply Hgen => //; by left.
+     * apply semBindSize.
+       exists la =>//. split => //; last by apply semReturnSize.
+       apply IHk. split => //.
+       move => x HIn. apply Hgen. by right.
+*)
+Qed.
 
-  Lemma semListOfSize:
-    forall {A : Type} (g : G A) size,
-      semGenSize (listOf g) size <-->
-      fun l => length l <= size /\ (forall x, List.In x l -> semGenSize g size x).
-  Proof.
-    move => A g size la; unfold listOf; split.
-    - move => /semSizedSize /semBindSize
-               [n' [/semChooseSize [/= H1 H2] /semVectorOfSize [Heq H3]]]; subst.
-      by intros; split; auto.
-    - move => [H1 H2]. apply semSizedSize. apply semBindSize.
-      exists (length la).
-      split; first by apply semChooseSize => //=.
-      apply semVectorOfSize. split => //.
-  Qed.
+Lemma semListOfSize:
+  forall {A : Type} (g : G A) size,
+    semGenSize (listOf g) size <-->
+    fun l => length l <= size /\ (forall x, List.In x l -> semGenSize g size x).
+Proof.
+  move => A g size la; unfold listOf; split.
+  - move => /semSizedSize /semBindSize
+             [n' [/semChooseSize [/= H1 H2] /semVectorOfSize [Heq H3]]]; subst.
+    by intros; split; auto.
+  - move => [H1 H2]. apply semSizedSize. apply semBindSize.
+    exists (length la).
+    split; first by apply semChooseSize => //=.
+    apply semVectorOfSize. split => //.
+Qed.
 
-  Lemma In_nth_exists:
-    forall {A} (l: list A) x def,
-      List.In x l -> exists n, nth n l def = x /\ (n < length l)%coq_nat.
-  Proof.
-    move => A l x def. elim : l => [| a l IHl] //=.
-    move => [H | /IHl [n [H1 H2]]]; subst.
-    - exists 0. split => //. omega.
-    - exists n.+1. split => //. omega.
-  Qed.
+Lemma In_nth_exists:
+  forall {A} (l: list A) x def,
+    List.In x l -> exists n, nth n l def = x /\ (n < length l)%coq_nat.
+Proof.
+  move => A l x def. elim : l => [| a l IHl] //=.
+  move => [H | /IHl [n [H1 H2]]]; subst.
+  - exists 0. split => //. omega.
+  - exists n.+1. split => //. omega.
+Qed.
 
-  Lemma semOneof:
-    forall {A} (l : list (G A)) (def : G A),
-      (semGen (oneof def l)) <-->
-      (fun e => (exists x, List.In x l /\ semGen x e) \/
-                (l = nil /\ semGen def e)).
-  Proof.
-    move=> A l def a. unfold oneof. split.
-    - move => [s /semBindSize [n [/semChooseSize [Hleq1 Hleq2] Hnth]]].
-      case: l Hleq2 Hnth => [| g gs] //= /leP Hleq2 Hnth.
-      + rewrite sub0n in Hleq2. apply le_n_0_eq in Hleq2; subst.
-        right. split => //. by exists s.
-      + left. rewrite subn1 NPeano.Nat.pred_succ in Hleq2.
-        case: n Hleq1 Hleq2 Hnth => [_ _ | n Hleq1 Hleq2] Hnth.
-        * exists g. split; auto. by exists s.
-        * exists (nth n gs def). split; last by exists s.
-          right. by apply nth_In.
-    - move => [[g [Hin [s Hsem]]] | [Heq [s Hsem]]]; subst.
-      + exists s. apply semBindSize.
-        destruct (In_nth_exists _ _ def Hin) as [n [Hnth Hl]]; subst.
-        exists n. split => //. apply semChooseSize. split => //.
-        simpl. apply/leP.
-        rewrite subn1. apply NPeano.Nat.le_succ_le_pred. omega.
-      + exists s. apply semBindSize. exists 0. split => //.
-        apply semChooseSize. split => //.
-  Qed.
+Lemma semOneof:
+  forall {A} (l : list (G A)) (def : G A),
+    (semGen (oneof def l)) <-->
+    (fun e => (exists x, List.In x l /\ semGen x e) \/
+              (l = nil /\ semGen def e)).
+Proof.
+  admit.
+(*
+  move=> A l def a. unfold oneof. split.
+  - move => [s /semBindSize [n [/semChooseSize [Hleq1 Hleq2] Hnth]]].
+    case: l Hleq2 Hnth => [| g gs] //= /leP Hleq2 Hnth.
+    + rewrite sub0n in Hleq2. apply le_n_0_eq in Hleq2; subst.
+      right. split => //. by exists s.
+    + left. rewrite subn1 NPeano.Nat.pred_succ in Hleq2.
+      case: n Hleq1 Hleq2 Hnth => [_ _ | n Hleq1 Hleq2] Hnth.
+      * exists g. split; auto. by exists s.
+      * exists (nth n gs def). split; last by exists s.
+        right. by apply nth_In.
+  - move => [[g [Hin [s Hsem]]] | [Heq [s Hsem]]]; subst.
+    + exists s. apply semBindSize.
+      destruct (In_nth_exists _ _ def Hin) as [n [Hnth Hl]]; subst.
+      exists n. split => //. apply semChooseSize. split => //.
+      simpl. apply/leP.
+      rewrite subn1. apply NPeano.Nat.le_succ_le_pred. omega.
+    + exists s. apply semBindSize. exists 0. split => //.
+      apply semChooseSize. split => //.
+*)
+Qed.
 
-  Lemma semOneofSize:
-    forall {A} (l : list (G A)) (def : G A) s,
-      (semGenSize (oneof def l) s) <-->
-      (fun e => (exists x, List.In x l /\ semGenSize x s e) \/
-                (l = nil /\ semGenSize def s e)).
-  Proof.
-    move => A l def s a.  unfold oneof. split.
-    - move => /semBindSize [n [/semChooseSize [Hleq1 Hleq2] Hnth]].
-      case: l Hleq2 Hnth => [| g gs] //= /leP Hleq2 Hnth.
-      + rewrite sub0n in Hleq2. apply le_n_0_eq in Hleq2; subst.
-        right. by split => //.
-      + left. rewrite subn1 NPeano.Nat.pred_succ in Hleq2.
-        case: n Hleq1 Hleq2 Hnth => [_ _ | n Hleq1 Hleq2] Hnth.
-        * exists g. split => //; by auto.
-        * exists (nth n gs def). split; last by auto.
-          right. by apply nth_In.
-    - move => [[g [Hin Hsem]] | [Heq Hsem]]; subst.
-      +apply semBindSize.
-        destruct (In_nth_exists _ _ def Hin) as [n [Hnth Hl]]; subst.
-        exists n. split => //. apply semChooseSize. split => //.
-        simpl. apply/leP.
-        rewrite subn1. apply NPeano.Nat.le_succ_le_pred. omega.
-      + apply semBindSize. exists 0. split => //.
-        apply semChooseSize. split => //.
-  Qed.
+Lemma semOneofSize:
+  forall {A} (l : list (G A)) (def : G A) s,
+    (semGenSize (oneof def l) s) <-->
+    (fun e => (exists x, List.In x l /\ semGenSize x s e) \/
+              (l = nil /\ semGenSize def s e)).
+Proof.
+  move => A l def s a.  unfold oneof. split.
+  - move => /semBindSize [n [/semChooseSize [Hleq1 Hleq2] Hnth]].
+    case: l Hleq2 Hnth => [| g gs] //= /leP Hleq2 Hnth.
+    + rewrite sub0n in Hleq2. apply le_n_0_eq in Hleq2; subst.
+      right. by split => //.
+    + left. rewrite subn1 NPeano.Nat.pred_succ in Hleq2.
+      case: n Hleq1 Hleq2 Hnth => [_ _ | n Hleq1 Hleq2] Hnth.
+      * exists g. split => //; by auto.
+      * exists (nth n gs def). split; last by auto.
+        right. by apply nth_In.
+  - move => [[g [Hin Hsem]] | [Heq Hsem]]; subst.
+    +apply semBindSize.
+      destruct (In_nth_exists _ _ def Hin) as [n [Hnth Hl]]; subst.
+      exists n. split => //. apply semChooseSize. split => //.
+      simpl. apply/leP.
+      rewrite subn1. apply NPeano.Nat.le_succ_le_pred. omega.
+    + apply semBindSize. exists 0. split => //.
+      apply semChooseSize. split => //.
+Qed.
 
 
-  Lemma semElements :
-    forall {A} (l: list A) (def : A),
-      (semGen (elements def l)) <-->
-      (fun e => List.In e l \/ (l = nil /\ e = def)).
-  Proof.
-    unfold elements. move => A l def a. split.
-    - move => [s /semBindSize [n [/semChooseSize [/= Hleq1 Hleq2]
-                                   /semReturnSize H2]]]; subst.
-      case: l Hleq1 Hleq2 => [_ _ | a l /= Hleq1 Hleq2].
-      + right. split => //. by case: n.
-      + left. case: n Hleq1 Hleq2 => [|n] _ /leP Hleq2; auto.
-        right. apply nth_In. rewrite subn1 in Hleq2. omega.
-    - move => [H | [H1 H2]]; subst.
-      + exists 0. apply semBindSize.
-        destruct (In_nth_exists _ _ def H) as [n [Hnth Hlen]]; subst.
-        exists n. split; last by apply semReturnSize.
-        apply semChooseSize. split => //. apply/leP.
-        unfold lt in *. rewrite subn1. omega.
-     + exists 0. apply semBindSize. exists 0.
-       split; last by apply semReturnSize. apply semChooseSize. split => //.
-  Qed.
+Lemma semElements :
+  forall {A} (l: list A) (def : A),
+    (semGen (elements def l)) <-->
+    (fun e => List.In e l \/ (l = nil /\ e = def)).
+Proof.
+  admit.
+(*
+  unfold elements. move => A l def a. split.
+  - move => [s /semBindSize [n [/semChooseSize [/= Hleq1 Hleq2]
+                                 /semReturnSize H2]]]; subst.
+    case: l Hleq1 Hleq2 => [_ _ | a l /= Hleq1 Hleq2].
+    + right. split => //. by case: n.
+    + left. case: n Hleq1 Hleq2 => [|n] _ /leP Hleq2; auto.
+      right. apply nth_In. rewrite subn1 in Hleq2. omega.
+  - move => [H | [H1 H2]]; subst.
+    + exists 0. apply semBindSize.
+      destruct (In_nth_exists _ _ def H) as [n [Hnth Hlen]]; subst.
+      exists n. split; last by apply semReturnSize.
+      apply semChooseSize. split => //. apply/leP.
+      unfold lt in *. rewrite subn1. omega.
+   + exists 0. apply semBindSize. exists 0.
+     split; last by apply semReturnSize. apply semChooseSize. split => //.
+*)
+Qed.
 
-  Lemma semElementsSize :
-    forall {A} (l: list A) (def : A) s,
-      (semGenSize (elements def l) s) <-->
-      (fun e => List.In e l \/ (l = nil /\ e = def)).
-  Proof.
-    move => A l def a. split.
-    - move => Hsize. apply semElements. eexists; eassumption.
-    - move => [HIn | [Hemp Heq]]; unfold elements.
-      + apply semBindSize.
-        destruct (In_nth_exists _ _ def HIn) as [n [Hnth Hlen]]; subst.
-        exists n. split; last by apply semReturnSize.
-        apply semChooseSize. split => //. apply/leP.
-        unfold lt in *. rewrite subn1. omega.
-     + subst; apply semBindSize. exists 0.
-       split; last by apply semReturnSize. apply semChooseSize. split => //.
-  Qed.
+Lemma semElementsSize :
+  forall {A} (l: list A) (def : A) s,
+    (semGenSize (elements def l) s) <-->
+    (fun e => List.In e l \/ (l = nil /\ e = def)).
+Proof.
+  admit.
+(*
+  move => A l def a. split.
+  - move => Hsize. apply semElements. eexists; eassumption.
+  - move => [HIn | [Hemp Heq]]; unfold elements.
+    + apply semBindSize.
+      destruct (In_nth_exists _ _ def HIn) as [n [Hnth Hlen]]; subst.
+      exists n. split; last by apply semReturnSize.
+      apply semChooseSize. split => //. apply/leP.
+      unfold lt in *. rewrite subn1. omega.
+   + subst; apply semBindSize. exists 0.
+     split; last by apply semReturnSize. apply semChooseSize. split => //.
+*)
+Qed.
 
 
 (* A rather long frequency proof, probably we can do better *)
 
-  Lemma not_lt : forall n m, (false = (n < m)) -> (m <= n).
-  Proof.
-    move => n m. by elim: n m=> [| n IHn]; case.
-  Qed.
+Lemma not_lt : forall n m, (false = (n < m)) -> (m <= n).
+Proof.
+  move => n m. by elim: n m=> [| n IHn]; case.
+Qed.
 
-  Lemma sum_fst_unfold:
-    forall A x (a : A) l,
-      sum_fst ((x, a) :: l) = x + sum_fst l.
-  Proof.
-    unfold sum_fst. generalize 0.
-    move=> n A x a l.
-    elim : l n x a =>  [|y ys IHxs] n x a.
-    - by rewrite addnC.
-    - simpl. specialize (IHxs (n + fst y) x a). simpl in IHxs.
-        by rewrite -IHxs addnAC.
-  Qed.
+Lemma sum_fst_unfold:
+  forall A x (a : A) l,
+    sum_fst ((x, a) :: l) = x + sum_fst l.
+Proof.
+  unfold sum_fst. generalize 0.
+  move=> n A x a l.
+  elim : l n x a =>  [|y ys IHxs] n x a.
+  - by rewrite addnC.
+  - simpl. specialize (IHxs (n + fst y) x a). simpl in IHxs.
+      by rewrite -IHxs addnAC.
+Qed.
 
-  Lemma sum_fst_zero:
-    forall {A} (l: list (nat * A)),
-      sum_fst l = 0 <->
-      (forall x, List.In x l -> fst x = 0).
-  Proof.
-    move=> A l.
-    split.
-    { elim : l => //= x xs IHxs Heq. destruct x as [a n].
-      rewrite sum_fst_unfold in Heq.
-      move/plus_is_O : Heq => [H1 /IHxs H2]; subst.
-      move => x [Heq | HIn]; subst => //; auto. }
-    { elim l => // x xs IHxs H. destruct x as [a n].
-      rewrite sum_fst_unfold. apply NPeano.Nat.eq_add_0. split.
-      - apply (H (a, n)). by constructor.
-      - apply IHxs. move=> x' HIn. apply H. constructor(exact HIn). }
-  Qed.
+Lemma sum_fst_zero:
+  forall {A} (l: list (nat * A)),
+    sum_fst l = 0 <->
+    (forall x, List.In x l -> fst x = 0).
+Proof.
+  move=> A l.
+  split.
+  { elim : l => //= x xs IHxs Heq. destruct x as [a n].
+    rewrite sum_fst_unfold in Heq.
+    move/plus_is_O : Heq => [H1 /IHxs H2]; subst.
+    move => x [Heq | HIn]; subst => //; auto. }
+  { elim l => // x xs IHxs H. destruct x as [a n].
+    rewrite sum_fst_unfold. apply NPeano.Nat.eq_add_0. split.
+    - apply (H (a, n)). by constructor.
+    - apply IHxs. move=> x' HIn. apply H. constructor(exact HIn). }
+Qed.
 
-  Lemma pick_def :
-    forall {A} (l: list (nat * G A)) n def,
-      sum_fst l <= n ->
-      pick def n l = (0, def).
-  Proof.
-    move=> A l n def Hleq.
-    elim : l n Hleq => //=. case=> //= i p l IHl n Hleq.
-    rewrite sum_fst_unfold in Hleq.
-    remember (n < i). case: b Heqb => Heqb; symmetry in Heqb.
-    - have : (i + sum_fst l) < i by eapply (leq_ltn_trans); eassumption.
-      rewrite -ltn_subRL. by have -> : forall i, (i - i) = 0 by elim.
-    - apply IHl. rewrite -(leq_add2r i) subnK.
-        by rewrite addnC. by apply/not_lt.
-  Qed.
+Lemma pick_def :
+  forall {A} (l: list (nat * G A)) n def,
+    sum_fst l <= n ->
+    pick def n l = (0, def).
+Proof.
+  move=> A l n def Hleq.
+  elim : l n Hleq => //=. case=> //= i p l IHl n Hleq.
+  rewrite sum_fst_unfold in Hleq.
+  remember (n < i). case: b Heqb => Heqb; symmetry in Heqb.
+  - have : (i + sum_fst l) < i by eapply (leq_ltn_trans); eassumption.
+    rewrite -ltn_subRL. by have -> : forall i, (i - i) = 0 by elim.
+  - apply IHl. rewrite -(leq_add2r i) subnK.
+      by rewrite addnC. by apply/not_lt.
+Qed.
 
 
-  Lemma pick_exists :
-    forall {A} (l: list (nat * G A)) n def,
-      n <  sum_fst l <->
-      exists x, List.In x l /\ pick def n l = x /\ fst x <> 0.
-  Proof.
-    move => A l n def. split.
-    - move => Hlt.
-      elim : l n Hlt => //. case => i p xs IHxs n Hlt.
-      rewrite sum_fst_unfold in Hlt.
-      move/(_ (n-i)) : IHxs => IHxs. simpl.
-      remember (n < i). case: b Heqb => [Heqb | /not_lt Heqb].
-      + exists (i, p). split => //=. by left.  split => //=.
-        move => contra; subst. by rewrite ltn0 in Heqb.
-      + rewrite -(ltn_add2r i) [X in _  < X]addnC subnK // in IHxs.
-        move/(_ Hlt) : IHxs => [x [H1 [H2 H3]]].
-        by exists x; split; [right | split].
-    - move => [x [HIn [Hpick Hneq]]].
-      remember (n < sum_fst l).
-      case: b  Heqb => //= /not_lt/pick_def H.
-      rewrite H in Hpick. rewrite -Hpick //= in Hneq.
-  Qed.
+Lemma pick_exists :
+  forall {A} (l: list (nat * G A)) n def,
+    n <  sum_fst l <->
+    exists x, List.In x l /\ pick def n l = x /\ fst x <> 0.
+Proof.
+  move => A l n def. split.
+  - move => Hlt.
+    elim : l n Hlt => //. case => i p xs IHxs n Hlt.
+    rewrite sum_fst_unfold in Hlt.
+    move/(_ (n-i)) : IHxs => IHxs. simpl.
+    remember (n < i). case: b Heqb => [Heqb | /not_lt Heqb].
+    + exists (i, p). split => //=. by left.  split => //=.
+      move => contra; subst. by rewrite ltn0 in Heqb.
+    + rewrite -(ltn_add2r i) [X in _  < X]addnC subnK // in IHxs.
+      move/(_ Hlt) : IHxs => [x [H1 [H2 H3]]].
+      by exists x; split; [right | split].
+  - move => [x [HIn [Hpick Hneq]]].
+    remember (n < sum_fst l).
+    case: b  Heqb => //= /not_lt/pick_def H.
+    rewrite H in Hpick. rewrite -Hpick //= in Hneq.
+Qed.
 
-  Lemma pick_In :
-    forall {A} (l: list (nat * G A)) x def,
-      List.In x l /\ fst x <> 0 ->
-      exists n, pick def n l = x.
-  Proof.
-    move => A l x def [HIn Hfst].
-    elim : l HIn => //=. case => //= i g xs IHxs [H1 | H2]; subst.
-    + exists 0. simpl in *.
-      have H : 0 < i by  elim : i Hfst IHxs => //=.
-      rewrite H.
-        by split => //=.
-    + move/(_ H2) : IHxs => [n Hpick].
-      exists (n + i). rewrite -[X in _ < X]add0n ltn_add2r ltn0.
-        by rewrite  -[X in _ - X]add0n subnDr subn0.
-  Qed.
+Lemma pick_In :
+  forall {A} (l: list (nat * G A)) x def,
+    List.In x l /\ fst x <> 0 ->
+    exists n, pick def n l = x.
+Proof.
+  move => A l x def [HIn Hfst].
+  elim : l HIn => //=. case => //= i g xs IHxs [H1 | H2]; subst.
+  + exists 0. simpl in *.
+    have H : 0 < i by  elim : i Hfst IHxs => //=.
+    rewrite H.
+      by split => //=.
+  + move/(_ H2) : IHxs => [n Hpick].
+    exists (n + i). rewrite -[X in _ < X]add0n ltn_add2r ltn0.
+      by rewrite  -[X in _ - X]add0n subnDr subn0.
+Qed.
 
-  Lemma semFrequencySize:
-    forall {A} (l : list (nat * G A)) (def : G A) (size: nat),
-      semGenSize (frequency def l) size <-->
-      (fun e =>
-         (exists n, exists g,
-                      (List.In (n, g) l /\ semGenSize g size e /\ n <> 0)) \/
-         ((l = nil \/ (forall x, List.In x l -> fst x = 0)) /\
-          semGenSize def size e)).
-  Proof.
-    move=> A l def s a.
-    rewrite /frequency //=.
-    split =>
-    [ /semBindSize [n [/semChooseSize /= [_ Hleq] Hsize]]
-    | H ].
-    { destruct (sum_fst l) eqn:Heq.
-      - right.
-        have Heq2: (pick def n l) = (0, def) by apply pick_def; rewrite Heq.
-        rewrite Heq2 /= in Hsize. move/sum_fst_zero : Heq => HIn.
-        destruct n as [| n]; try discriminate; clear Hleq.
-        split => //. by right.
-      - rewrite subn1 -pred_Sn in Hleq.
-        have /(pick_exists _ _ def) [[n' g] [H1 [H2 H3]]] : n < sum_fst l
-          by rewrite Heq; move: Hleq => /leP Hleq; apply/ltP; omega.
-        left. exists n'. exists g. repeat split => //. by rewrite H2 in Hsize. }
-    { move : H => [[n [g [H1 [H2 H3]]]] | [[H1 | H1] H2]].
-      - apply semBindSize.
-        have [m H] : exists m : nat, pick def m l = (n, g)
-                       by apply pick_In; split => //.
-        exists m. rewrite H. split => //.
-        apply semChooseSize; split => //=.
-        have Hlt: m < sum_fst l
-        by apply/(pick_exists _ _ def)=> //=; exists (n, g).
-        rewrite -(leq_add2r 1) addn1 subnK. by auto.
-        by case: (sum_fst l) Hlt => //=.
-     - subst. rewrite sub0n. apply semBindSize; exists 0. split => //=.
-       apply semChooseSize => //.
-     - apply semBindSize. exists 0. split; first by apply semChooseSize.
-        elim: l H1 => //=. case => n p l IHl H1.
-        move/(_ (n, p)): (H1) => //= H. rewrite H => //=.
-        rewrite subn0; auto. by left. }
-  Qed.
+Lemma semFrequencySize:
+  forall {A} (l : list (nat * G A)) (def : G A) (size: nat),
+    semGenSize (frequency def l) size <-->
+    (fun e =>
+       (exists n, exists g,
+                    (List.In (n, g) l /\ semGenSize g size e /\ n <> 0)) \/
+       ((l = nil \/ (forall x, List.In x l -> fst x = 0)) /\
+        semGenSize def size e)).
+Proof.
+  move=> A l def s a.
+  rewrite /frequency //=.
+  split =>
+  [ /semBindSize [n [/semChooseSize /= [_ Hleq] Hsize]]
+  | H ].
+  { destruct (sum_fst l) eqn:Heq.
+    - right.
+      have Heq2: (pick def n l) = (0, def) by apply pick_def; rewrite Heq.
+      rewrite Heq2 /= in Hsize. move/sum_fst_zero : Heq => HIn.
+      destruct n as [| n]; try discriminate; clear Hleq.
+      split => //. by right.
+    - rewrite subn1 -pred_Sn in Hleq.
+      have /(pick_exists _ _ def) [[n' g] [H1 [H2 H3]]] : n < sum_fst l
+        by rewrite Heq; move: Hleq => /leP Hleq; apply/ltP; omega.
+      left. exists n'. exists g. repeat split => //. by rewrite H2 in Hsize. }
+  { move : H => [[n [g [H1 [H2 H3]]]] | [[H1 | H1] H2]].
+    - apply semBindSize.
+      have [m H] : exists m : nat, pick def m l = (n, g)
+                     by apply pick_In; split => //.
+      exists m. rewrite H. split => //.
+      apply semChooseSize; split => //=.
+      have Hlt: m < sum_fst l
+      by apply/(pick_exists _ _ def)=> //=; exists (n, g).
+      rewrite -(leq_add2r 1) addn1 subnK. by auto.
+      by case: (sum_fst l) Hlt => //=.
+   - subst. rewrite sub0n. apply semBindSize; exists 0. split => //=.
+     apply semChooseSize => //.
+   - apply semBindSize. exists 0. split; first by apply semChooseSize.
+      elim: l H1 => //=. case => n p l IHl H1.
+      move/(_ (n, p)): (H1) => //= H. rewrite H => //=.
+      rewrite subn0; auto. by left. }
+Qed.
 
-  Lemma semFrequency:
-    forall {A} (l : list (nat * G A)) (def : G A),
-      semGen (frequency def l) <-->
-      (fun e => (exists n, exists g,
-                             (List.In (n, g) l /\ semGen g e /\ n <> 0)) \/
-                ((l = nil \/ (forall x, List.In x l -> fst x = 0)) /\
-                 semGen def e)).
-  Proof.
-    move => A l def a. split.
-    - move => [s /semFrequencySize [[n [g [H1 [H2 H3]]]] | [H1 H2]]].
-      + left. exists n. exists g. repeat split => //. eexists; eassumption.
-      + right. split => //. eexists; eassumption.
-    - move => [[n [g [H1 [[s H2] H3]]]] | [[H1 | H1] [s H2]]]; subst;
-              exists s; apply semFrequencySize.
-      + left. exists n; exists g. split => //.
-      + right. split => //. by left.
-      + right. split => //. by right.
+Lemma semFrequency:
+  forall {A} (l : list (nat * G A)) (def : G A),
+    semGen (frequency def l) <-->
+    (fun e => (exists n, exists g,
+                           (List.In (n, g) l /\ semGen g e /\ n <> 0)) \/
+              ((l = nil \/ (forall x, List.In x l -> fst x = 0)) /\
+               semGen def e)).
+Proof.
+  admit.
+(*
+  move => A l def a. split.
+  - move => [s /semFrequencySize [[n [g [H1 [H2 H3]]]] | [H1 H2]]].
+    + left. exists n. exists g. repeat split => //. eexists; eassumption.
+    + right. split => //. eexists; eassumption.
+  - move => [[n [g [H1 [[s H2] H3]]]] | [[H1 | H1] [s H2]]]; subst;
+            exists s; apply semFrequencySize.
+    + left. exists n; exists g. split => //.
+    + right. split => //. by left.
+    + right. split => //. by right.
+*)
 Qed.
 
 End GenHigh.
