src/Sets.v
@@ -1,0 +1,230 @@
+Require Import ssreflect ssrfun ssrbool ssrnat.
+Require Import Classes.RelationClasses Classes.Morphisms.
+(*
+Require Import Random RoseTrees.
+Require Import Ensembles.
+Require Import Numbers.BinNums.
+*)
+
+Set Implicit Arguments.
+Unset Strict Implicit.
+Unset Printing Implicit Defensive.
+
+(*
+Import ListNotations.
+*)
+
+(* Low-level Generators *)
+
+(* There are similar definitions in the Ensembles library (Included
+   and Same_set); set_eq is not exactly the same as Same_set though
+   (only logically equivalent). *)
+
+Definition set T := T -> Prop.
+
+Notation "x \in A" := (A x) (at level 70, only parsing) : set_scope.
+
+Definition set_eq {A} (m1 m2 : set A) :=
+  forall (a : A), m1 a <-> m2 a.
+
+Global Instance : forall T, Equivalence (@set_eq T).
+Proof. admit. Qed.
+
+Infix "<-->" := set_eq (at level 70, no associativity) : set_scope.
+
+Definition set_incl {A} (m1 m2 : set A) :=
+  forall (a : A), m1 a -> m2 a.
+
+Infix "\subset" := set_incl (at level 70, no associativity) : set_scope.
+
+Open Scope set_scope.
+
+Notation "[ 'set' x : T | P ]" := (fun x : T => P)
+  (at level 0, x at level 99, only parsing) : set_scope.
+Notation "[ 'set' x | P ]" := [set x : _ | P]
+  (at level 0, x, P at level 99, format "[ 'set'  x  |  P ]", only parsing) : set_scope.
+
+Definition setT {T} := [set _ : T | True].
+
+Notation "[ 'set' : T ]" := (@setT T)
+  (at level 0, format "[ 'set' :  T ]") : set_scope.
+
+Section setOpsDef.
+
+Context {T U : Type}.
+Implicit Types (a x : T) (A B : set T).
+
+Definition set1 a := eq a.
+
+Definition setU A B := [set x | x \in A \/ x \in B].
+
+Definition setI A B := [set x | x \in A /\ x \in B].
+
+Definition codom (f : T -> U) := [set y | exists x, f x = y].
+
+Definition bigcup A (F : T -> set U) := [set x | exists i, i \in A /\ x \in F i].
+
+End setOpsDef.
+
+Definition imset {T U} (f : T -> U) A := bigcup A (fun x => set1 (f x)).
+
+Definition setX T U (A : set T) (B : set U) := [set x | x.1 \in A /\ x.2 \in B].
+
+Definition imset2 T U V (f : T -> U -> V) A1 A2 :=
+  imset (prod_curry f) (setX A1 A2).
+
+Definition codom2 T U V (f : T -> U -> V) := codom (prod_curry f).
+
+Notation "[ 'set' a ]" := (set1 a)
+  (at level 0, a at level 99, format "[ 'set'  a ]") : set_scope.
+Notation "[ 'set' a : T ]" := [set (a : T)]
+  (at level 0, a at level 99, format "[ 'set'  a   :  T ]") : set_scope.
+
+Notation "A :|: B" := (setU A B) (at level 52, left associativity) : set_scope.
+Notation "a |: A" := ([set a] :|: A) (at level 52, left associativity) : set_scope.
+
+Notation "A :&: B" := (setI A B) (at level 48, left associativity) : set_scope.
+
+Notation "f @: A" := (imset f A) (at level 24) : set_scope.
+
+Notation "f @2: ( A , B )" := (imset2 f A B)
+  (at level 24, format "f  @2:  ( A ,  B )") : set_scope.
+
+Notation "\bigcup_ i F" := (bigcup setT (fun i => F))
+  (at level 41, F at level 41, i at level 0,
+           format "'[' \bigcup_ i '/  '  F ']'") : set_scope.
+Notation "\bigcup_ ( i : t ) F" := (bigcup (@setT t) (fun i => F))
+  (at level 41, F at level 41, i at level 50,
+           format "'[' \bigcup_ ( i   :  t ) '/  '  F ']'", only parsing) : set_scope.
+Notation "\bigcup_ ( i 'in' A ) F" := (bigcup A (fun i => F))
+  (at level 41, F at level 41, i, A at level 50,
+           format "'[' \bigcup_ ( i  'in'  A ) '/  '  F ']'") : set_scope.
+
+Lemma subset_eqP T (A B : set T) : (A <--> B) <-> (A \subset B /\ B \subset A).
+Proof.
+split; first by move=> eqAB; split=> a; rewrite (eqAB a).
+by case=> subAB subBA a; split; [apply: subAB | apply:subBA].
+Qed.
+
+Lemma imsetT T U (f : T -> U) : f @: setT <--> codom f.
+Proof.
+move=> y; split; first by case=> x [_ fx]; exists x.
+by case=> x fx; exists x.
+Qed.
+
+Instance set_incl_Proper T U :
+  Proper (@eq (T -> U) ==> set_incl ==> set_incl) imset.
+Proof.
+by move=> f ? <- A B subAB y [x [Ax fx]]; exists x; split=> //; apply: subAB.
+Qed.
+
+Instance set_eq_Proper T U : Proper (@eq (T -> U) ==> set_eq ==> set_eq) imset.
+Proof.
+by move=> f ? <- A B /subset_eqP[subAB subBA] y; split; apply: set_incl_Proper.
+Qed.
+
+Lemma bigcup_set1 T U (F : T -> set U) y :
+  \bigcup_(x in [set y]) F x <--> F y.
+Proof. by move=> t; split=> [[y' [<-]] | Fyt] //; exists y. Qed.
+
+Lemma bigcup_const A B (P : set B) : inhabited A -> (\bigcup_(_ : A) P) <--> P.
+Proof. by case=> a x; split=> [[?] []|Px] //; exists a. Qed.
+
+Lemma bigcupC T U V A B (F : T -> U -> set V) :
+  \bigcup_(i in A) \bigcup_(j in B) F i j <-->
+  \bigcup_(j in B) \bigcup_(i in A) F i j.
+Proof.
+wlog suff: T U A B F / \bigcup_(i in A) \bigcup_(j in B) F i j \subset
+   \bigcup_(j in B) \bigcup_(i in A) F i j.
+  by move=> sub; apply/subset_eqP; split; apply: sub.
+by move=> x [i [Ai [j [Bj ?]]]]; exists j; split=> //; exists i.
+Qed.
+
+Lemma incl_bigcupr T U A (F : T -> set U) G : (forall x, F x \subset G x) ->
+  \bigcup_(x in A) F x \subset \bigcup_(x in A) G x.
+Proof.
+by move=> subFG t [x [Ax Fxt]]; exists x; split=> //; apply: subFG.
+Qed.
+
+Lemma eq_bigcupr T U A (F : T -> set U) G : (forall x, F x <--> G x) ->
+  \bigcup_(x in A) F x <--> \bigcup_(x in A) G x.
+Proof.
+by move=> eq_FG t; split; apply: incl_bigcupr => {t} x t; rewrite (eq_FG x t).
+Qed.
+
+Lemma incl_bigcupl T U A B (F : T -> set U) : A \subset B ->
+  \bigcup_(x in A) F x \subset \bigcup_(x in B) F x.
+Proof.
+by move=> subAB t [x [Ax Fxt]]; exists x; split=> //; apply: subAB.
+Qed.
+
+Global Instance eq_bigcupl T U : Proper (set_eq ==> @eq (T -> set U) ==> set_eq) bigcup.
+Proof.
+by move=> A B /subset_eqP[? ?] F G <- {G}; split; apply: incl_bigcupl.
+Qed.
+
+Lemma bigcup_flatten T U V A (F : T -> set U) (G : U -> set V) :
+  \bigcup_(x in \bigcup_(y in A) F y) G x <-->
+  \bigcup_(y in A) \bigcup_(x in F y) G x.
+Proof.
+move=> t; split=> [[x [[y [Ay Fyx]] Gxt]] | [y [Ay [x [Fyx Gxt]]]]].
+  by exists y; split=> //; exists x.
+by exists x; split=> //; exists y.
+Qed.
+
+Lemma codomE T U (f : T -> U) : codom f <--> \bigcup_x [set f x].
+Proof. by move=> y; split=> [[x fx]|[x [_ fx]]]; exists x. Qed.
+
+Lemma codom_id T : codom id <--> [set: T].
+Proof. by move=> x; split=> // _; exists x. Qed.
+
+Lemma codom_const A B (x : B) : inhabited A ->
+  codom (fun _ : A => x) <--> [set x].
+Proof. by move=> ?; rewrite codomE bigcup_const. Qed.
+
+Lemma imset_comp T U V (f : U -> T) (g : V -> U) A :
+  (f \o g) @: A <--> f @: (g @: A).
+Proof.
+by rewrite /imset bigcup_flatten; apply: eq_bigcupr => x; rewrite bigcup_set1.
+Qed.
+
+Lemma codom_comp T U V (f : U -> T) (g : V -> U) :
+  codom (f \o g) <--> f @: (codom g).
+Proof. by rewrite -imsetT imset_comp imsetT. Qed.
+
+Lemma curry_imset2l T U V (f : T -> U -> V) A1 A2 :
+  f @2: (A1, A2) <--> \bigcup_(x1 in A1) f x1 @: A2.
+Proof.
+move=> a; split.
+  by case=> [[x1 x2] [[/= Ax1 Ax2] fx]]; exists x1; split=> //; exists x2.
+by case=> [x1 [Ax1 [x2 [Ax2 fx]]]]; exists (x1,x2).
+Qed.
+
+Lemma curry_imset2r T U V (f : T -> U -> V) A1 A2 :
+  f @2: (A1, A2) <--> \bigcup_(x2 in A2) f^~ x2 @: A1.
+Proof. by rewrite curry_imset2l bigcupC. Qed.
+
+Lemma curry_codom2l T U V (f : T -> U -> V) :
+  codom (prod_curry f) <--> \bigcup_x1 codom (f x1).
+Proof.
+admit.
+Qed.
+
+Lemma imset_bigcup T U V (f : U -> V) A (F : T -> set U) :
+  (f @: \bigcup_(x in A) (F x)) <--> \bigcup_(x in A) f @: F x.
+Proof. by rewrite /imset bigcup_flatten. Qed.
+
+Lemma bigcup_imset T U V (f : T -> U) A (F : U -> set V) :
+  \bigcup_(y in f @: A) (F y) <--> \bigcup_(x in A) F (f x).
+Proof.
+by rewrite bigcup_flatten; apply: eq_bigcupr => x; rewrite bigcup_set1.
+Qed.
+
+Lemma bigcup_codom T U V (f : T -> U) (F : U -> set V) :
+  \bigcup_(y in codom f) (F y) <--> \bigcup_x F (f x).
+Proof.
+admit.
+Qed.
+
+Lemma coverE T : \bigcup_x [set x] <--> [set: T].
+Proof. by rewrite -codomE codom_id. Qed.
